lexicographic recursion version of evaluate

cakeSemantics/CakeAST.v
@@ -70,113 +70,71 @@ Inductive fptop : Type :=
 
 
 Inductive op : Type :=
-  | Opn : opn -> op
-  | Opb : opb -> op
-  | Opw : word_size -> opw -> op
-  | Shift : word_size -> shift -> nat -> op
-  | Equality : op
-  (* Floating point is currently not supported and
-   * only included for translation purposes *)
-  | OpFpCmp : fpcmp -> op
-  | OpFpUop : fpuop -> op
-  | OpFpBop : fpbop -> op
-  | OpFpTop : fptop -> op
-  | Opapp : op
-  | Opassign : op
-  | Opref : op
-  | Opderef : op
-  | Aw8alloc : op
-  | Aw8sub : op
-  | Aw8length : op
-  | Aw8update : op
-  | WordFromInt : word_size -> op
-  | WordToInt : word_size -> op
-  | CopyStrStr : op
-  | CopyStrAw8 : op
-  | CopyAw8Str : op
-  | CopyAw8Aw8 : op
-
-  | Ord : op
-  | Chr : op
-  | Chopb : opb -> op
-  | Implode : op
-  | Explode : op
-  | Strsub : op
-  | Strlen : op
-  | Strcat : op
-  | VfromList : op
-  | Vsub : op
-  | Vlength : op
-  | Aalloc : op
-  | AallocEmpty : op
-  | Asub : op
-  | Alength : op
-  | Aupdate : op
-  | ListAppend : op
-  | ConfigGC : op
-  | FFI : string -> op.
+  | Opapp : op.
 
 Inductive lop : Type :=
   | And : lop
   | Or : lop.
-
-(* Inductive Forall' (A : Type) (P' : A -> Set) : list A -> Set := *)
-(* | Forall_nil' : Forall' A P' [] *)
-(* | Forall_cons' : forall (x : A) (l : list A), P' x -> Forall' A P' l -> Forall' A P' (x :: l). *)
-
-(* LATER: replace using LibList function *)
 
 (* Helper relation for lists *)
 Inductive Forall'' (A : Type) (P'' : A -> Type) : list A -> Type :=
 | Forall_nil'' : Forall'' A P'' []
 | Forall_cons'' : forall (x : A) (l : list A), P'' x -> Forall'' A P'' l -> Forall'' A P'' (x :: l).
 
+Arguments Forall'' {A } _.
+
+(* Definition Forall'' {A : Type} (P : A -> Type) (l : list A) := forall (a : A), In a l -> P a. *)
+
 (* We need to build our own inductive principles for a bit *)
 Unset Elimination Schemes.
-(* Set Elimination Schemes. *)
-(* Patterns *)
-
-(* Types *)
 
 (** BACKPORT this definition to Cakeml Lem semantics *)
 Definition constr_id : Type :=
   option (ident modN conN).
 
 Inductive ast_t : Type :=
-  | Atvar : tvarN -> ast_t
-  | Atfun : ast_t -> ast_t -> ast_t
-  | Attup : list ast_t -> ast_t
   | Atapp : list ast_t -> ident modN typeN -> ast_t.
 
 Inductive pat : Type :=
-  | Pany : pat
   | Pvar : varN -> pat
-  | Plit : lit -> pat
-  | Pcon : constr_id -> list pat -> pat
-  | Pref : pat -> pat
-  | Ptannot : pat -> ast_t -> pat.
+  | Pcon : constr_id -> list pat -> pat.
 
 (* locs Defined elsewhere in the Lem spec *)
 Definition locs : Type := list nat.
 
 (* Expressions *)
 Inductive exp : Type :=
-  | ERaise : exp -> exp
-  | EHandle : exp -> list (pat * exp) -> exp
-  | ELit : lit -> exp
   | ECon : constr_id -> list exp -> exp
   | EVar : ident modN varN -> exp
   | EFun : varN -> exp -> exp
   | EApp : op -> list exp -> exp
-  | ELog : lop -> exp -> exp -> exp
-  | EIf  : exp -> exp -> exp -> exp
   | EMat : exp -> list (pat * exp) -> exp
-  | ELet : option varN -> exp -> exp -> exp
-  | ELetrec : list (varN * varN * exp) -> exp -> exp
-  | ETannot : exp -> ast_t -> exp
   | ELannot : exp -> locs -> exp.
 
-Hint Constructors exp.
+Set Elimination Schemes.
+
+(* Inductive is_subexp : exp -> list exp -> Prop := *)
+(* | ReflexiveSubexp : forall (e : exp), is_subexp e [e] *)
+(* | ListSubexp : forall (e e' : exp) (l : list exp), *)
+(*     is_subexp e [e'] \/ is_subexp e l -> *)
+(*     is_subexp e (e'::l) *)
+(* | ECon_subexp : forall (cid : constr_id) (e : exp) (l : list exp), *)
+(*     is_subexp e l -> *)
+(*     is_subexp e [ECon cid l] *)
+(* | EFun_subexp : forall (v : varN) (e1 e2 : exp), *)
+(*     is_subexp e1 [e2] -> *)
+(*     is_subexp e1 [EFun v e2] *)
+(* | EApp_subexp : forall (e : exp) (o : op) (l : list exp), *)
+(*     is_subexp e l -> *)
+(*     is_subexp e [EApp o l] *)
+(* | EMat_subexp : forall (e1 e2 : exp) (l : list (pat * exp)), *)
+(*     is_subexp e1 [e2] \/ is_subexp e1 (map snd l) -> *)
+(*     is_subexp e1 [EMat e2 l] *)
+(* | ELannot_subexp : forall (e1 e2 : exp) (lcs : locs), *)
+(*     is_subexp e1 [e2] -> *)
+(*     is_subexp e1 [ELannot e2 lcs]. *)
+
+Unset Elimination Schemes.
 
 Definition typeDef : Type :=
   list (list tvarN * typeN * list (conN * list ast_t)).
@@ -185,104 +143,50 @@ Definition typeDef : Type :=
 Inductive dec : Type :=
   | Dlet : locs -> pat -> exp -> dec
   | Dletrec : locs -> list (varN * varN * exp) -> dec
-  | Dtype : locs -> typeDef -> dec
-  | Dtabbrev : locs -> list tvarN -> typeN -> ast_t -> dec
-  | Dexn : locs -> conN -> list ast_t -> dec
-  | Dmod : modN -> list dec -> dec
-  | Dlocal : list dec -> list dec -> dec.
-
-
-(** BACKPORT the new definition without accumulator
-
-Fixpoint pat_bindings (p : pat) (already_bound : list varN) : list varN :=
-  let fix pats_bindings (ps : list pat) (already_bound : list varN) : list varN :=
-      match ps with
-      | [] => already_bound
-      | p::ps => pats_bindings ps (pat_bindings p already_bound)
-      end
-  in
-  match p with
-  | Pany => already_bound
-  | Pvar n => n :: already_bound
-  | Plit l => already_bound
-  | Pcon _ ps => pats_bindings ps already_bound
-  | Pref p => pat_bindings p already_bound
-  | Ptannot p _ => pat_bindings p already_bound
-  end.
-
-*)
+  | Dtype : locs -> typeDef -> dec.
 
 Fixpoint pat_bindings (p : pat) : list varN :=
   match p with
-  | Pany => []
   | Pvar n => n :: []
-  | Plit l => []
   | Pcon _ ps => List.fold_right (fun p acc => acc ++ pat_bindings p) [] ps
-  | Pref p => pat_bindings p
-  | Ptannot p _ => pat_bindings p
   end.
 
 
 (*-------------------------------------------------------------------*)
 (** Begin induction principle *)
 
-(* LATER: could use List.fold_right function *)
-
 (** AST *)
-
 Fixpoint ast_t_rect (P : ast_t -> Type)
-         (H1 : forall (t : tvarN), P (Atvar t))
-         (H2 : forall (a1 a2 : ast_t), P a1 -> P a2 -> P (Atfun a1 a2))
-         (H3 : forall (l : list ast_t), Forall'' ast_t P l -> P (Attup l))
-         (H4 : forall (l : list ast_t) (i : ident modN typeN), Forall'' ast_t P l -> P (Atapp l i))
+         (H1 : forall (l : list ast_t) (i : ident modN typeN), Forall'' P l -> P (Atapp l i))
          (a : ast_t) : P a :=
   match a with
-  | Atvar t => H1 t
-  | Atfun a1 a2 => H2 a1 a2 (ast_t_rect P H1 H2 H3 H4 a1) (ast_t_rect P H1 H2 H3 H4 a2)
-  | Attup l => let fix F (ls : list ast_t) :=
-                   match ls with
-                   | [] => Forall_nil'' ast_t P
-                   | h::t => Forall_cons'' ast_t P h t (ast_t_rect P H1 H2 H3 H4 h) (F t)
-                   end
-               in H3 l (F l)
   | Atapp l i => let fix F (ls : list ast_t) :=
                    match ls with
                    | [] => Forall_nil'' ast_t P
-                   | h::t => Forall_cons'' ast_t P h t (ast_t_rect P H1 H2 H3 H4 h) (F t)
+                   | h::t => Forall_cons'' ast_t P h t (ast_t_rect P H1 h) (F t)
                    end
-               in H4 l i (F l)
+               in H1 l i (F l)
   end.
 
 Definition ast_t_ind (P : ast_t -> Prop) := ast_t_rect P.
 Definition ast_t_rec (P : ast_t -> Set) := ast_t_rect P.
 
-
 (** PAT *)
 
 Fixpoint pat_rect (P : pat -> Type)
-         (H1 : P Pany)
-         (H2 : forall (v : varN), P (Pvar v))
-         (H3 : forall (l : lit), P (Plit l))
-         (H4 : forall (o : constr_id) (l : list pat), Forall'' pat P l -> P (Pcon o l))
-         (H5 : forall (p : pat), P p -> P (Pref p))
-         (H6 : forall (p : pat), P p -> forall (a : ast_t), P (Ptannot p a))
+         (H1 : forall (v : varN), P (Pvar v))
+         (H2 : forall (o : constr_id) (l : list pat), Forall'' P l -> P (Pcon o l))
          (p : pat) : P p :=
   match p return (P p) with
-  | Pany => H1
-  | Pvar v => H2 v
-  | Plit l => H3 l
+  | Pvar v => H1 v
   | Pcon o l => let fix loop (l : list pat) :=
                    match l with
                    | [] => Forall_nil'' pat P
-                   | h::t => Forall_cons'' pat P h t (pat_rect P H1 H2 H3 H4 H5 H6 h) (loop t)
+                   | h::t => Forall_cons'' pat P h t (pat_rect P H1 H2 h) (loop t)
                    end
                in
-               H4 o l (loop l)
-  | Pref p'  => H5 p' (pat_rect P H1 H2 H3 H4 H5 H6 p')
-  | Ptannot p' a => H6 p' (pat_rect P H1 H2 H3 H4 H5 H6 p') a
+               H2 o l (loop l)
   end.
-
-(* LATER: above could use List.fold_right function *)
 
 Definition pat_rec (P : pat -> Set) := pat_rect P.
 Definition pat_ind (P : pat -> Prop) := pat_rect P.
@@ -301,26 +205,16 @@ Definition exp_rect_helper' (P : exp -> Type) (p : varN * varN * exp) : Type :=
   end.
 
 Fixpoint exp_rect (P : exp -> Type)
-         (H1 : forall (e : exp), P e -> P (ERaise e))
-         (H2 : forall (e : exp), P e -> forall (l : list (pat * exp)), Forall'' (pat * exp) (exp_rect_helper P) l
-                                                            -> P (EHandle e l))
-         (H3 : forall (l : lit), P (ELit l))
-         (H4 : forall (o : constr_id) (l : list exp), Forall'' exp P l
+         (H1 : forall (o : constr_id) (l : list exp), Forall'' P l
                                                                 -> P (ECon o l))
-         (H5 : forall (i : ident modN varN), P (EVar i))
-         (H6 : forall (v : varN) (e : exp), P e -> P (EFun v e))
-         (H7 : forall (o : op) (l : list exp), Forall'' exp P l -> P (EApp o l))
-         (H8 : forall (l : lop) (e1 e2 : exp), P e1 -> P e2 -> P (ELog l e1 e2))
-         (H9 : forall (e1 e2 e3 : exp), P e1 -> P e2 -> P e3 -> P (EIf e1 e2 e3))
-         (H10 : forall (e : exp), P e -> forall (l : list (pat * exp)), Forall'' (pat * exp) (exp_rect_helper P) l
+         (H2 : forall (i : ident modN varN), P (EVar i))
+         (H3 : forall (v : varN) (e : exp), P e -> P (EFun v e))
+         (H4 : forall (o : op) (l : list exp), Forall'' P l -> P (EApp o l))
+         (H5 : forall (e : exp), P e -> forall (l : list (pat * exp)), Forall'' (exp_rect_helper P) l
                                                              -> P (EMat e l))
-         (H11 : forall (o : option varN) (e1 e2 : exp), P e1 -> P e2 -> P (ELet o e1 e2))
-         (H12 : forall (l : list (varN * varN * exp)), Forall'' (varN * varN * exp) (exp_rect_helper' P) l
-                                                  -> forall (e : exp), P e -> P (ELetrec l e))
-         (H13 : forall (e : exp) (a : ast_t), P e -> P (ETannot e a))
-         (H14 : forall (e : exp) (l : locs), P e -> P (ELannot e l))
+         (H6 : forall (e : exp) (l : locs), P e -> P (ELannot e l))
          (e : exp) : P e :=
-  let exp_rect' := fun e' => exp_rect P H1 H2 H3 H4 H5 H6 H7 H8 H9 H10 H11 H12 H13 H14 e' in
+  let exp_rect' := fun e' => exp_rect P H1 H2 H3 H4 H5 H6 e' in
   let fix loop (l : list exp) :=
       match l with
       | [] => Forall_nil'' exp P
@@ -340,25 +234,16 @@ Fixpoint exp_rect (P : exp -> Type)
       end
   in
   match e with
-  | ERaise e' => H1 e' (exp_rect' e')
-  | EHandle e' l => H2 e' (exp_rect' e') l (pair_loop l)
-  | ELit l    => H3 l
-  | ECon o l  => H4 o l (loop l)
-  | EVar i    => H5 i
-  | EFun v e' => H6 v e' (exp_rect' e')
-  | EApp o l  => H7 o l (loop l)
-  | ELog l e1 e2 => H8 l e1 e2 (exp_rect' e1) (exp_rect' e2)
-  | EIf  e1 e2 e3 => H9 e1 e2 e3 (exp_rect' e1) (exp_rect' e2) (exp_rect' e3)
-  | EMat e' l     => H10 e' (exp_rect' e') l (pair_loop l)
-  | ELet o e1 e2  => H11 o e1 e2 (exp_rect' e1) (exp_rect' e2)
-  | ELetrec l e'  => H12 l (trip_loop l) e' (exp_rect' e')
-  | ETannot e' a  => H13 e' a (exp_rect' e')
-  | ELannot e' l  => H14 e' l (exp_rect' e')
+  | ECon o l  => H1 o l (loop l)
+  | EVar i    => H2 i
+  | EFun v e' => H3 v e' (exp_rect' e')
+  | EApp o l  => H4 o l (loop l)
+  | EMat e' l     => H5 e' (exp_rect' e') l (pair_loop l)
+  | ELannot e' l  => H6 e' l (exp_rect' e')
   end.
 
 Definition exp_rec (P : exp -> Set) := exp_rect P.
 Definition exp_ind (P : exp -> Prop) := exp_rect P.
-
 
 (** DEC *)
 
@@ -366,31 +251,11 @@ Fixpoint dec_rect (P : dec -> Type)
          (H1 : forall (l : locs) (p : pat) (e : exp), P (Dlet l p e))
          (H2 : forall (l : locs) (lv : list (varN * varN * exp)), P (Dletrec l lv))
          (H3 : forall (l : locs) (t : typeDef), P (Dtype l t))
-         (H4 : forall (l : locs) (lt : list tvarN) (t : typeN) (a : ast_t), P (Dtabbrev l lt t a))
-         (H5 : forall (l : locs) (c : conN) (la : list ast_t), P (Dexn l c la))
-         (H6 : forall (m : modN) (l : list dec), Forall'' dec P l -> P (Dmod m l))
-         (H7 : forall (l0 : list dec) (l1 : list dec), Forall'' dec P l0 -> Forall'' dec P l1 -> P (Dlocal l0 l1))
          (d : dec) : P d :=
   match d with
   | Dlet l p e => H1 l p e
   | Dletrec l lv => H2 l lv
   | Dtype l t => H3 l t
-  | Dtabbrev l lt t a => H4 l lt t a
-  | Dexn l c la => H5 l c la
-  | Dmod m l => let fix loop (l : list dec) :=
-                   match l with
-                   | [] => Forall_nil'' dec P
-                   | h::t => Forall_cons'' dec P h t (dec_rect P H1 H2 H3 H4 H5 H6 H7 h) (loop t)
-                   end
-               in
-               H6 m l (loop l)
-  | Dlocal l0 l1 => let fix loop (l : list dec) :=
-                       match l with
-                       | [] => Forall_nil'' dec P
-                       | h::t => Forall_cons'' dec P h t (dec_rect P H1 H2 H3 H4 H5 H6 H7 h) (loop t)
-                       end
-                   in
-               H7 l0 l1 (loop l0) (loop l1)
   end.
 
 Definition dec_rec (P : dec -> Set) := dec_rect P.
@@ -437,15 +302,14 @@ Hint Resolve lop_eq_dec : DecidableEquality.
 Theorem ast_t_eq_dec : forall (a1 a2 : ast_t), {a1 = a2} + {a1 <> a2}.
 Proof.
   decide equality; auto with DecidableEquality; try (apply ident_eq_dec; apply string_dec);
-  generalize dependent l0;
-  induction H; destruct l0;
+  generalize dependent l0.
+  induction l; destruct l0;
     try (left; reflexivity);
-    try (right; discriminate);
-    try (destruct (p a);
-         destruct (IHForall'' l0);
-         try (inversion e0);
-         try (right; intro con; injection con; contradiction);
-         rewrite e; left; reflexivity).
+    try (right; discriminate).
+  inv H.
+  destruct (H2 a0); destruct (IHl H3 l0);
+    try (left; congruence);
+    try (right; congruence).
 Defined.
 Hint Resolve ast_t_eq_dec : DecidableEquality.
 
@@ -457,13 +321,11 @@ Hint Resolve constr_id_eq_dec : DecidableEquality.
 Theorem pat_eq_dec : forall (p0 p1 : pat), {p0 = p1} + {p0 <> p1}.
 Proof. decide equality; auto with DecidableEquality.
        generalize dependent l0.
-         induction l; destruct l0; try (left; reflexivity); try (right; discriminate).
+       induction l; destruct l0; try (left; reflexivity); try (right; discriminate).
        inv X.
-       destruct (X0 p); subst.
-       destruct (IHl X1 l0); subst.
-       - left; reflexivity.
-       - right; intro con; inversion con; auto.
-       - right; intro con; inversion con; auto.
+       destruct (X0 p); destruct (IHl X1 l0);
+         try (left; congruence);
+         try (right; congruence).
 Defined.
 Hint Resolve pat_eq_dec : DecidableEquality.
 
@@ -480,48 +342,45 @@ Proof.
 Defined.
 Hint Resolve locs_eq_dec : DecidableEquality.
 
+
 Theorem exp_eq_dec : forall (e0 e1 : exp), {e0 = e1} + {e0 <> e1}.
 Proof.
   decide equality; auto with DecidableEquality;
     try (decide equality; try (apply ident_eq_dec); apply string_dec); generalize dependent l0.
 
-  induction X0; destruct l0.
-  - left; reflexivity.
-  - right; discriminate.
-  - right; discriminate.
-  - destruct x; destruct p0; simpl in *.
-    destruct (pat_eq_dec p1 p0); destruct (p e4); destruct (IHX0 l0); subst;
-      try (right; injection; auto); (left; reflexivity).
-  - induction X; destruct l0; try (left; reflexivity); try (right; discriminate).
-    destruct (p e); destruct (IHX l0); subst; try (right; injection; auto); left; reflexivity.
-  - induction X; destruct l0; try (left; reflexivity); try (right; discriminate).
-    destruct (p e); destruct (IHX l0); subst; try (right; injection; auto); left; reflexivity.
-  - induction X0; destruct l0; try (left; reflexivity); try (right; discriminate).
-    destruct x; destruct p0; simpl in *.
-    destruct (p e4); destruct (pat_eq_dec p1 p0); destruct (IHX0 l0); subst;
-      try (right; injection; auto); left; reflexivity.
-  - induction X; destruct l0; try (left; reflexivity); try (right; discriminate).
-    destruct x as [x' xe]; destruct x' as [xv0 xv1];
-      destruct p0 as [p0' p0e]; destruct p0' as [p0v0 p0v1]; simpl in *.
-    destruct (p p0e); destruct (string_dec xv0 p0v0); destruct (string_dec xv1 p0v1); destruct (IHX l0); subst;
-      try (right; injection; auto); left; reflexivity.
-Defined.
+  - induction l; destruct l0.
+    + left; reflexivity.
+    + right; congruence.
+    + right; congruence.
+    + inv X.
+      destruct (X0 e); destruct (IHl X1 l0);
+        try (left; congruence);
+        try (right; congruence).
+
+  - induction l; destruct l0.
+    + left; reflexivity.
+    + right; congruence.
+    + right; congruence.
+    + inv X; subst.
+      * destruct (X0 e); destruct (IHl X1 l0); subst;
+          try (left; reflexivity);
+          try (right; congruence).
+  - induction l; destruct l0;
+      try (left; reflexivity);
+      try (right; congruence).
+    inv X0.
+    destruct a0 as [ap ae]; destruct p as [pp pe]; destruct (pat_eq_dec ap pp);
+      destruct (X1 pe); destruct (IHl X2 l0); subst;
+        try (left; reflexivity);
+        try (right; congruence).
+Qed.
+
 Hint Resolve exp_eq_dec : DecidableEquality.
 
 Theorem dec_eq_dec : forall (d0 d1 : dec), {d0 = d1} + {d0 <> d1}.
 Proof.
   decide equality; try (auto with DecidableEquality).
-  - generalize dependent l0. induction X; destruct l0; try (left; reflexivity); try (right; discriminate).
-    destruct (p d); destruct (IHX l0); subst; try (right; injection; auto); left; reflexivity.
-  - generalize dependent l2. induction X0; destruct l2; try (left; reflexivity); try (right; discriminate).
-    destruct (p d); destruct (IHX0 l2); subst; try (right; injection; auto); left; reflexivity.
-  - generalize dependent l; induction X.
-    + destruct l.
-      * left; reflexivity.
-      * right; discriminate.
-    + destruct l0.
-      * right; discriminate.
-      * destruct (p d); destruct (IHX l0); subst; try (right; injection; auto); left; reflexivity.
 Defined.
 Hint Resolve dec_eq_dec : DecidableEquality.
+
 (*-------------------------------------------------------------------*)
