cakeSemantics/Evaluate.v
@@ -81,16 +81,16 @@ Fixpoint pmatch (envC : env_ctor) (s : store val) (p : pat) (v : val)
       end
   in
   match p, v with
-  | Pany, v' => Match env
+  (* | Pany, v' => Match env *)
   | Pvar x, v' => Match ((x,v')::env)
-  | Plit l, Litv l' => if lit_eq_dec l l'
-                      then Match env
-                      else if lit_same_type l l'
-                           then No_match
-                           else Match_type_error
+  (* | Plit l, Litv l' => if lit_eq_dec l l' *)
+  (*                     then Match env *)
+  (*                     else if lit_same_type l l' *)
+  (*                          then No_match *)
+  (*                          else Match_type_error *)
   | Pcon (Some n) ps, Conv (Some stamp') vs =>
     match  nsLookup ident_string_dec n envC with
-    | Some (l, stamp) =>  if same_ctor stamp stamp'
+    | Some (l, stamp) =>  if stamp_eq_dec stamp stamp'
                          then if eq_nat_dec (length ps) l (* TODO: suspicious redundant test *)
                               then pmatch_list envC s ps vs env
                               else Match_type_error
@@ -104,12 +104,12 @@ Fixpoint pmatch (envC : env_ctor) (s : store val) (p : pat) (v : val)
   (* if eqb (length ps) (length vs) *)
   (* then pmatch_list envC s ps vs env *)
   (* else Match_type_error *)
-  | Pref p, Loc lnum => match store_lookup lnum s with
-                       | Some (Refv v) => pmatch envC s p v env
-                       | Some _ => Match_type_error
-                       | None => Match_type_error
-                       end
-  | Ptannot p t, val' => pmatch envC s p val' env
+  (* | Pref p, Loc lnum => match store_lookup lnum s with *)
+  (*                      | Some (Refv v) => pmatch envC s p v env *)
+  (*                      | Some _ => Match_type_error *)
+  (*                      | None => Match_type_error *)
+  (*                      end *)
+  (* | Ptannot p t, val' => pmatch envC s p val' env *)
   | _, _ => Match_type_error
   end.
 
@@ -203,15 +203,15 @@ Fixpoint do_opapp (vs : list val) : option (sem_env val * exp) :=
 Definition store_ffi (ffi' : Type) (V : Type) := (store V * ffi_state ffi')%type.
 
 Definition natFromInteger (size : nat) :=
-      let fix helper (n' : nat ) (z : Z) : nat :=
-          match n' with
-          | O => O
-          | S n'' =>
-            (2 ^ n' * (Z.to_nat (Zdigits.bit_value
-                                            (Z.testbit (Z.of_nat n'') z)))
-                          + (helper n'' z))
-          end
-      in helper size.
+  let fix helper (n' : nat ) (z : Z) : nat :=
+      match n' with
+      | O => O
+      | S n'' =>
+        (2 ^ n' * (Z.to_nat (Zdigits.bit_value
+                               (Z.testbit (Z.of_nat n'') z)))
+             + (helper n'' z))
+      end
+  in helper size.
 
 Definition word8FromInteger (i : Z) : word 8 := nat_to_word 8 (natFromInteger 8 i)%nat .
 Definition word64FromInteger (i : Z) : word 64 :=  nat_to_word 64 (natFromInteger 64%nat i).
@@ -221,256 +221,256 @@ Fixpoint do_app (ffi' : Type) (st : store_ffi ffi' val) (o : op) (vs : list val)
   match st with
     (s, t) =>
     match o, vs with
-    | ListAppend, [x1;x2] =>
-      match val_to_list x1, val_to_list x2 with
-      | Some xs, Some ys =>
-        Some ((s,t), Rval (list_to_val (xs ++ ys)))
-      | _, _ => None
-      end
-    | Opn o', [Litv (IntLit n1); Litv (IntLit n2)] =>
-      if sumbool_and _ _ _ _ (Z.eq_dec n2 0) (sumbool_or _ _ _ _ (opn_eq_dec o' Divide) (opn_eq_dec o' Modulo))
-        then Some ((s,t), Rerr (Rraise div_exn_v))
-        else Some ((s,t), Rval (Litv (IntLit (opn_lookup o' n1 n2))))
-    | Opb o', [Litv (IntLit n1); Litv (IntLit n2)] =>
-      Some ((s,t), Rval (Boolv (opb_lookup o' n1 n2)))
-    | Opw W8 o', [Litv (Word8Lit w1); Litv (Word8Lit w2)] =>
-      Some ((s,t), Rval (Litv (Word8Lit (opw8_lookup o' w1 w2))))
-    | Opw W64 o', [Litv (Word64Lit w1); Litv (Word64Lit w2)] =>
-      Some ((s,t), Rval (Litv (Word64Lit (opw64_lookup o' w1 w2))))
-    (* | FP_bop bop, [Litv (Word64Lit w1); Litv (Word64Lit w2)] => *)
-    (*     Some ((s,t),Rval (Litv (Word64Lit (fp_bop bop w1 w2)))) *)
-    (* | FP_uop uop, [Litv (Word64Lit w)] => *)
-    (*   Some ((s,t),Rval (Litv (Word64Lit (fp_uop uop w)))) *)
-    (* | FP_cmp cmp, [Litv (Word64Lit w1); Litv (Word64Lit w2)] => *)
-    (*   Some ((s,t),Rval (Boolv (fp_cmp cmp w1 w2))) *)
-    | Shift W8 o' n, [Litv (Word8Lit w)] =>
-      Some ((s,t), Rval (Litv (Word8Lit (shift8_lookup o' w n))))
-    | Shift W64 o' n, [Litv (Word64Lit w)] =>
-      Some ((s,t), Rval (Litv (Word64Lit (shift64_lookup o' w n))))
-    | Equality, [v1; v2] =>
-      match do_eq v1 v2 with
-      | Eq_type_error => None
-      | Eq_val b => Some ((s,t), Rval (Boolv b))
-      end
-    | Opassign, [Loc lnum; v] =>
-      match store_assign lnum (Refv v) s with
-      | Some s' => Some ((s',t), Rval (Conv None []))
-      | None => None
-      end
-    | Opref, [v] =>
-      let (s',n) := store_alloc (Refv v) s in
-      Some ((s',t), Rval (Loc n))
-    | Opderef, [Loc n] =>
-      match store_lookup n s with
-      | Some (Refv v) => Some ((s,t), Rval v)
-      | _ => None
-      end
-    | Aw8alloc, [Litv (IntLit n); Litv (Word8Lit w)] =>
-      if (Z_lt_dec n 0)%Z then
-        Some ((s,t), Rerr (Rraise sub_exn_v))
-      else
-        let (s',lnum) := store_alloc (W8array (List.repeat w (Z.to_nat n))) s
-        in Some ((s',t), Rval (Loc lnum))
-    | Aw8sub, [Loc lnum; Litv (IntLit i)] =>
-      match store_lookup lnum s with
-      | Some (W8array ws) =>
-        if (Z_lt_dec i 0)%Z
-        then Some ((s,t), Rerr (Rraise sub_exn_v))
-        else
-          let n := Z.to_nat i in
-          match List.nth_error ws n with
-          | None => Some ((s,t), Rerr (Rraise sub_exn_v))
-          | Some n' => Some ((s,t), Rval (Litv (Word8Lit n')))
-          end
-      | _ => None
-      end
-    | Aw8length, [Loc n] =>
-      match store_lookup n s with
-      | Some (W8array ws) => Some ((s,t), Rval (Litv (IntLit (ZArith.Zcomplements.Zlength ws))))
-      | _ => None
-      end
-    | Aw8update, [Loc lnum; Litv (IntLit i); Litv (Word8Lit w)] =>
-      match store_lookup lnum s with
-      | Some (W8array ws) =>
-        if (Z_lt_dec i 0)%Z then
-          Some ((s,t), Rerr (Rraise sub_exn_v))
-        else
-          let n := Z.to_nat i in
-          if Nat.leb (List.length ws) n then
-            Some ((s,t), Rerr (Rraise sub_exn_v))
-          else
-            match store_assign lnum (W8array (update n w ws)) s with
-            | None => None
-            | Some s' => Some ((s',t), Rval (Conv None []))
-            end
-      | _ => None
-      end
-    | WordFromInt W8, [Litv (IntLit i)] =>
-      Some ((s,t), Rval (Litv (Word8Lit (word8FromInteger i))))
-    | WordFromInt W64, [Litv (IntLit i)] =>
-      Some ((s,t), Rval (Litv (Word64Lit (word64FromInteger i))))
-    | WordToInt W8, [Litv (Word8Lit w)] =>
-      Some ((s,t), Rval (Litv (IntLit (Z.of_nat (word_to_nat _ w)))))
-    | WordToInt W64, [Litv (Word64Lit w)] =>
-      Some ((s,t), Rval (Litv (IntLit (Z.of_nat (word_to_nat _ w)))))
-    | CopyStrStr, [Litv (StrLit str); Litv (IntLit off); Litv (IntLit len)] =>
-      Some ((s,t),
-            match copy_array (string_to_list_char str,off) len None with
-            | None => Rerr (Rraise sub_exn_v)
-            | Some cs => Rval (Litv (StrLit (list_char_to_string cs)))
-            end)
-    | CopyStrAw8, [Litv (StrLit str); Litv (IntLit off); Litv (IntLit len);
-                     Loc dst; Litv (IntLit dstoff)] =>
-      match store_lookup dst s with
-      | Some (W8array ws) =>
-        match copy_array (string_to_list_char str, off) len
-                         (Some (map word8_to_char ws, dstoff)) with
-        | None => Some ((s,t), Rerr (Rraise sub_exn_v))
-        | Some cs =>
-          match store_assign dst (W8array (map char_to_word8 cs)) s with
-          | Some s' =>  Some ((s',t), Rval (Conv None []))
-          | _ => None
-          end
-        end
-      | _ => None
-      end
-    | CopyAw8Str, [Loc src; Litv (IntLit off); Litv (IntLit len)] =>
-      match store_lookup src s with
-      | Some (W8array ws) =>
-        Some ((s,t),
-        match copy_array (ws,off) len None with
-        | None => Rerr (Rraise sub_exn_v)
-        | Some ws => Rval (Litv (StrLit( list_char_to_string
-                                         (map word8_to_char ws))))
-        end)
-      | _ => None
-      end
-    | CopyAw8Aw8, [Loc src; Litv (IntLit off); Litv (IntLit len);
-                     Loc dst; Litv (IntLit dstoff)] =>
-      match store_lookup src s, store_lookup dst s with
-      | Some (W8array ws), Some (W8array ds) =>
-        match copy_array (ws,off) len (Some (ds,dstoff)) with
-        | None => Some ((s,t), Rerr (Rraise sub_exn_v))
-        | Some ws =>
-          match store_assign dst (W8array ws) s with
-          | Some s' => Some ((s',t), Rval (Conv None []))
-          | _ => None
-          end
-        end
-      | _, _ => None
-      end
-    | Ord, [Litv (CharLit c)] =>
-      Some ((s,t), Rval (Litv (IntLit (Z.of_nat (nat_of_ascii c)))))
-    | Chr, [Litv (IntLit i)] =>
-      Some ((s,t), if sumbool_and _ _ _ _ (Z_lt_dec i 0)%Z (Z_lt_dec 255 i)%Z
-                   then Rerr (Rraise chr_exn_v)
-                   else Rval (Litv (CharLit (ascii_of_nat (Z.to_nat i)))))
-    | Chopb op, [Litv (CharLit c1); Litv (CharLit c2)] =>
-      Some ((s,t), Rval (Boolv (opb_lookup op (Z.of_nat (nat_of_ascii c1))
-                                           (Z.of_nat (nat_of_ascii c2)))))
-    | Implode, [v] =>
-      match val_to_char_list v with
-      | Some ls => Some ((s,t), Rval (Litv (StrLit (list_char_to_string ls))))
-      | None => None
-      end
-    | Strsub, [Litv (StrLit str); Litv (IntLit i)] =>
-      if (Z_lt_dec i 0)%Z then
-        Some ((s,t), Rerr (Rraise sub_exn_v))
-      else
-        let n := Z.to_nat i in
-        match String.get n str with
-        | Some n' => Some ((s,t), Rval (Litv (CharLit n')))
-        | None    => Some ((s,t), Rerr (Rraise sub_exn_v))
-        end
-    | StrLen, [Litv (StrLit str)] =>
-      Some ((s,t), Rval (Litv (IntLit (Z.of_nat (String.length str)))))
-    | Strcat, [v] =>
-      match val_to_list v with
-      | Some vs =>
-        match vals_to_string vs with
-        | Some str =>
-          Some ((s,t), Rval (Litv(StrLit str)))
-        | _ => None
-        end
-      | _ => None
-      end
-    | VfromList, [v] =>
-      match val_to_list v with
-      | Some vs => Some ((s,t), Rval (Vectorv vs))
-      | None    => None
-      end
-    | VSub, [Vectorv vs; Litv (IntLit i)] =>
-      if (Z_lt_dec i 0)%Z
-      then Some ((s,t), Rerr (Rraise sub_exn_v))
-      else
-        let n := Z.to_nat i in
-        match nth_error vs n with
-        | None    => Some ((s,t), Rerr (Rraise sub_exn_v))
-        | Some v' => Some ((s,t), Rval v')
-        end
-    | Vlength, [Vectorv vs] =>
-      Some ((s,t), Rval (Litv (IntLit (Z.of_nat (List.length  vs)))))
-    | Aalloc, [Litv (IntLit n); v] =>
-      if (Z_lt_dec n 0)%Z
-      then Some ((s,t), Rerr (Rraise sub_exn_v))
-      else
-        let (s',lnum) := store_alloc (Varray (List.repeat v (Z.to_nat n))) s
-        in Some ((s',t), Rval (Loc lnum))
-    | AallocEmpty, [Conv None []] =>
-      let (s',lnum) := store_alloc (Varray []) s
-      in Some ((s',t), Rval (Loc lnum))
-    | Asub, [Loc lnum; Litv (IntLit i)] =>
-      match store_lookup lnum s with
-      | Some (Varray vs) =>
-        if (Z_lt_dec i 0)%Z then
-          Some ((s,t), Rerr (Rraise sub_exn_v))
-        else
-          let n := Z.to_nat i in
-          match nth_error vs n with
-          | None    => Some ((s,t), Rerr (Rraise sub_exn_v))
-          | Some v' => Some ((s,t), Rval v')
-          end
-      | _ => None
-      end
-    | Alength, [Loc n] =>
-      match store_lookup n s with
-      | Some (Varray ws) =>
-        Some ((s,t), Rval (Litv (IntLit (Z.of_nat (List.length ws)))))
-      | _ => None
-      end
-    | Aupdate, [Loc lnum; Litv (IntLit i); v] =>
-      match store_lookup lnum s with
-      | Some (Varray vs') =>
-        if (Z_lt_dec i 0)%Z then (* LATER: use a wrapper function for this kind of test *)
-          Some ((s,t), Rerr (Rraise sub_exn_v))
-        else
-          let n := Z.to_nat i in
-          if Nat.leb (List.length vs') n
-          then Some ((s,t), Rerr (Rraise sub_exn_v))
-          else
-            match store_assign lnum (Varray (update n v vs')) s with
-            | None => None
-            | Some s' => Some ((s',t), Rval (Conv None []))
-            end
-      | _ => None
-      end
-    | ConfigGC, [Litv (IntLit i); Litv (IntLit j)] =>
-      Some ((s,t), Rval (Conv None []))
-    | FFI n, [Litv(StrLit conf); Loc lnum] =>
-      match store_lookup lnum s with
-      | Some (W8array ws) =>
-        match call_FFI t n (List.map (fun c' => nat_to_word 8 (nat_of_ascii c'))
-                                     (string_to_list_char conf)) ws with
-        | Ffi_return _ t' ws' =>
-          match store_assign lnum (W8array ws') s with
-          | Some s' => Some ((s', t'), Rval (Conv None []))
-          | None => None
-          end
-        | Ffi_final _ outcome =>
-          Some ((s, t), Rerr (Rabort (Rffi_error outcome)))
-        end
-      | _ => None
-      end
+    (* | ListAppend, [x1;x2] => *)
+    (*   match val_to_list x1, val_to_list x2 with *)
+    (*   | Some xs, Some ys => *)
+    (*     Some ((s,t), Rval (list_to_val (xs ++ ys))) *)
+    (*   | _, _ => None *)
+    (*   end *)
+    (* | Opn o', [Litv (IntLit n1); Litv (IntLit n2)] => *)
+    (*   if sumbool_and _ _ _ _ (Z.eq_dec n2 0) (sumbool_or _ _ _ _ (opn_eq_dec o' Divide) (opn_eq_dec o' Modulo)) *)
+    (*     then Some ((s,t), Rerr (Rraise div_exn_v)) *)
+    (*     else Some ((s,t), Rval (Litv (IntLit (opn_lookup o' n1 n2)))) *)
+    (* | Opb o', [Litv (IntLit n1); Litv (IntLit n2)] => *)
+    (*   Some ((s,t), Rval (Boolv (opb_lookup o' n1 n2))) *)
+    (* | Opw W8 o', [Litv (Word8Lit w1); Litv (Word8Lit w2)] => *)
+    (*   Some ((s,t), Rval (Litv (Word8Lit (opw8_lookup o' w1 w2)))) *)
+    (* | Opw W64 o', [Litv (Word64Lit w1); Litv (Word64Lit w2)] => *)
+    (*   Some ((s,t), Rval (Litv (Word64Lit (opw64_lookup o' w1 w2)))) *)
+    (* (* | FP_bop bop, [Litv (Word64Lit w1); Litv (Word64Lit w2)] => *) *)
+    (* (*     Some ((s,t),Rval (Litv (Word64Lit (fp_bop bop w1 w2)))) *) *)
+    (* (* | FP_uop uop, [Litv (Word64Lit w)] => *) *)
+    (* (*   Some ((s,t),Rval (Litv (Word64Lit (fp_uop uop w)))) *) *)
+    (* (* | FP_cmp cmp, [Litv (Word64Lit w1); Litv (Word64Lit w2)] => *) *)
+    (* (*   Some ((s,t),Rval (Boolv (fp_cmp cmp w1 w2))) *) *)
+    (* | Shift W8 o' n, [Litv (Word8Lit w)] => *)
+    (*   Some ((s,t), Rval (Litv (Word8Lit (shift8_lookup o' w n)))) *)
+    (* | Shift W64 o' n, [Litv (Word64Lit w)] => *)
+    (*   Some ((s,t), Rval (Litv (Word64Lit (shift64_lookup o' w n)))) *)
+    (* | Equality, [v1; v2] => *)
+    (*   match do_eq v1 v2 with *)
+    (*   | Eq_type_error => None *)
+    (*   | Eq_val b => Some ((s,t), Rval (Boolv b)) *)
+    (*   end *)
+    (* | Opassign, [Loc lnum; v] => *)
+    (*   match store_assign lnum (Refv v) s with *)
+    (*   | Some s' => Some ((s',t), Rval (Conv None [])) *)
+    (*   | None => None *)
+    (*   end *)
+    (* | Opref, [v] => *)
+    (*   let (s',n) := store_alloc (Refv v) s in *)
+    (*   Some ((s',t), Rval (Loc n)) *)
+    (* | Opderef, [Loc n] => *)
+    (*   match store_lookup n s with *)
+    (*   | Some (Refv v) => Some ((s,t), Rval v) *)
+    (*   | _ => None *)
+    (*   end *)
+    (* | Aw8alloc, [Litv (IntLit n); Litv (Word8Lit w)] => *)
+    (*   if (Z_lt_dec n 0)%Z then *)
+    (*     Some ((s,t), Rerr (Rraise sub_exn_v)) *)
+    (*   else *)
+    (*     let (s',lnum) := store_alloc (W8array (List.repeat w (Z.to_nat n))) s *)
+    (*     in Some ((s',t), Rval (Loc lnum)) *)
+    (* | Aw8sub, [Loc lnum; Litv (IntLit i)] => *)
+    (*   match store_lookup lnum s with *)
+    (*   | Some (W8array ws) => *)
+    (*     if (Z_lt_dec i 0)%Z *)
+    (*     then Some ((s,t), Rerr (Rraise sub_exn_v)) *)
+    (*     else *)
+    (*       let n := Z.to_nat i in *)
+    (*       match List.nth_error ws n with *)
+    (*       | None => Some ((s,t), Rerr (Rraise sub_exn_v)) *)
+    (*       | Some n' => Some ((s,t), Rval (Litv (Word8Lit n'))) *)
+    (*       end *)
+    (*   | _ => None *)
+    (*   end *)
+    (* | Aw8length, [Loc n] => *)
+    (*   match store_lookup n s with *)
+    (*   | Some (W8array ws) => Some ((s,t), Rval (Litv (IntLit (ZArith.Zcomplements.Zlength ws)))) *)
+    (*   | _ => None *)
+    (*   end *)
+    (* | Aw8update, [Loc lnum; Litv (IntLit i); Litv (Word8Lit w)] => *)
+    (*   match store_lookup lnum s with *)
+    (*   | Some (W8array ws) => *)
+    (*     if (Z_lt_dec i 0)%Z then *)
+    (*       Some ((s,t), Rerr (Rraise sub_exn_v)) *)
+    (*     else *)
+    (*       let n := Z.to_nat i in *)
+    (*       if Nat.leb (List.length ws) n then *)
+    (*         Some ((s,t), Rerr (Rraise sub_exn_v)) *)
+    (*       else *)
+    (*         match store_assign lnum (W8array (update n w ws)) s with *)
+    (*         | None => None *)
+    (*         | Some s' => Some ((s',t), Rval (Conv None [])) *)
+    (*         end *)
+    (*   | _ => None *)
+    (*   end *)
+    (* | WordFromInt W8, [Litv (IntLit i)] => *)
+    (*   Some ((s,t), Rval (Litv (Word8Lit (word8FromInteger i)))) *)
+    (* | WordFromInt W64, [Litv (IntLit i)] => *)
+    (*   Some ((s,t), Rval (Litv (Word64Lit (word64FromInteger i)))) *)
+    (* | WordToInt W8, [Litv (Word8Lit w)] => *)
+    (*   Some ((s,t), Rval (Litv (IntLit (Z.of_nat (word_to_nat _ w))))) *)
+    (* | WordToInt W64, [Litv (Word64Lit w)] => *)
+    (*   Some ((s,t), Rval (Litv (IntLit (Z.of_nat (word_to_nat _ w))))) *)
+    (* | CopyStrStr, [Litv (StrLit str); Litv (IntLit off); Litv (IntLit len)] => *)
+    (*   Some ((s,t), *)
+    (*         match copy_array (string_to_list_char str,off) len None with *)
+    (*         | None => Rerr (Rraise sub_exn_v) *)
+    (*         | Some cs => Rval (Litv (StrLit (list_char_to_string cs))) *)
+    (*         end) *)
+    (* | CopyStrAw8, [Litv (StrLit str); Litv (IntLit off); Litv (IntLit len); *)
+    (*                  Loc dst; Litv (IntLit dstoff)] => *)
+    (*   match store_lookup dst s with *)
+    (*   | Some (W8array ws) => *)
+    (*     match copy_array (string_to_list_char str, off) len *)
+    (*                      (Some (map word8_to_char ws, dstoff)) with *)
+    (*     | None => Some ((s,t), Rerr (Rraise sub_exn_v)) *)
+    (*     | Some cs => *)
+    (*       match store_assign dst (W8array (map char_to_word8 cs)) s with *)
+    (*       | Some s' =>  Some ((s',t), Rval (Conv None [])) *)
+    (*       | _ => None *)
+    (*       end *)
+    (*     end *)
+    (*   | _ => None *)
+    (*   end *)
+    (* | CopyAw8Str, [Loc src; Litv (IntLit off); Litv (IntLit len)] => *)
+    (*   match store_lookup src s with *)
+    (*   | Some (W8array ws) => *)
+    (*     Some ((s,t), *)
+    (*     match copy_array (ws,off) len None with *)
+    (*     | None => Rerr (Rraise sub_exn_v) *)
+    (*     | Some ws => Rval (Litv (StrLit( list_char_to_string *)
+    (*                                      (map word8_to_char ws)))) *)
+    (*     end) *)
+    (*   | _ => None *)
+    (*   end *)
+    (* | CopyAw8Aw8, [Loc src; Litv (IntLit off); Litv (IntLit len); *)
+    (*                  Loc dst; Litv (IntLit dstoff)] => *)
+    (*   match store_lookup src s, store_lookup dst s with *)
+    (*   | Some (W8array ws), Some (W8array ds) => *)
+    (*     match copy_array (ws,off) len (Some (ds,dstoff)) with *)
+    (*     | None => Some ((s,t), Rerr (Rraise sub_exn_v)) *)
+    (*     | Some ws => *)
+    (*       match store_assign dst (W8array ws) s with *)
+    (*       | Some s' => Some ((s',t), Rval (Conv None [])) *)
+    (*       | _ => None *)
+    (*       end *)
+    (*     end *)
+    (*   | _, _ => None *)
+    (*   end *)
+    (* | Ord, [Litv (CharLit c)] => *)
+    (*   Some ((s,t), Rval (Litv (IntLit (Z.of_nat (nat_of_ascii c))))) *)
+    (* | Chr, [Litv (IntLit i)] => *)
+    (*   Some ((s,t), if sumbool_and _ _ _ _ (Z_lt_dec i 0)%Z (Z_lt_dec 255 i)%Z *)
+    (*                then Rerr (Rraise chr_exn_v) *)
+    (*                else Rval (Litv (CharLit (ascii_of_nat (Z.to_nat i))))) *)
+    (* | Chopb op, [Litv (CharLit c1); Litv (CharLit c2)] => *)
+    (*   Some ((s,t), Rval (Boolv (opb_lookup op (Z.of_nat (nat_of_ascii c1)) *)
+    (*                                        (Z.of_nat (nat_of_ascii c2))))) *)
+    (* | Implode, [v] => *)
+    (*   match val_to_char_list v with *)
+    (*   | Some ls => Some ((s,t), Rval (Litv (StrLit (list_char_to_string ls)))) *)
+    (*   | None => None *)
+    (*   end *)
+    (* | Strsub, [Litv (StrLit str); Litv (IntLit i)] => *)
+    (*   if (Z_lt_dec i 0)%Z then *)
+    (*     Some ((s,t), Rerr (Rraise sub_exn_v)) *)
+    (*   else *)
+    (*     let n := Z.to_nat i in *)
+    (*     match String.get n str with *)
+    (*     | Some n' => Some ((s,t), Rval (Litv (CharLit n'))) *)
+    (*     | None    => Some ((s,t), Rerr (Rraise sub_exn_v)) *)
+    (*     end *)
+    (* | StrLen, [Litv (StrLit str)] => *)
+    (*   Some ((s,t), Rval (Litv (IntLit (Z.of_nat (String.length str))))) *)
+    (* | Strcat, [v] => *)
+    (*   match val_to_list v with *)
+    (*   | Some vs => *)
+    (*     match vals_to_string vs with *)
+    (*     | Some str => *)
+    (*       Some ((s,t), Rval (Litv(StrLit str))) *)
+    (*     | _ => None *)
+    (*     end *)
+    (*   | _ => None *)
+    (*   end *)
+    (* | VfromList, [v] => *)
+    (*   match val_to_list v with *)
+    (*   | Some vs => Some ((s,t), Rval (Vectorv vs)) *)
+    (*   | None    => None *)
+    (*   end *)
+    (* | VSub, [Vectorv vs; Litv (IntLit i)] => *)
+    (*   if (Z_lt_dec i 0)%Z *)
+    (*   then Some ((s,t), Rerr (Rraise sub_exn_v)) *)
+    (*   else *)
+    (*     let n := Z.to_nat i in *)
+    (*     match nth_error vs n with *)
+    (*     | None    => Some ((s,t), Rerr (Rraise sub_exn_v)) *)
+    (*     | Some v' => Some ((s,t), Rval v') *)
+    (*     end *)
+    (* | Vlength, [Vectorv vs] => *)
+    (*   Some ((s,t), Rval (Litv (IntLit (Z.of_nat (List.length  vs))))) *)
+    (* | Aalloc, [Litv (IntLit n); v] => *)
+    (*   if (Z_lt_dec n 0)%Z *)
+    (*   then Some ((s,t), Rerr (Rraise sub_exn_v)) *)
+    (*   else *)
+    (*     let (s',lnum) := store_alloc (Varray (List.repeat v (Z.to_nat n))) s *)
+    (*     in Some ((s',t), Rval (Loc lnum)) *)
+    (* | AallocEmpty, [Conv None []] => *)
+    (*   let (s',lnum) := store_alloc (Varray []) s *)
+    (*   in Some ((s',t), Rval (Loc lnum)) *)
+    (* | Asub, [Loc lnum; Litv (IntLit i)] => *)
+    (*   match store_lookup lnum s with *)
+    (*   | Some (Varray vs) => *)
+    (*     if (Z_lt_dec i 0)%Z then *)
+    (*       Some ((s,t), Rerr (Rraise sub_exn_v)) *)
+    (*     else *)
+    (*       let n := Z.to_nat i in *)
+    (*       match nth_error vs n with *)
+    (*       | None    => Some ((s,t), Rerr (Rraise sub_exn_v)) *)
+    (*       | Some v' => Some ((s,t), Rval v') *)
+    (*       end *)
+    (*   | _ => None *)
+    (*   end *)
+    (* | Alength, [Loc n] => *)
+    (*   match store_lookup n s with *)
+    (*   | Some (Varray ws) => *)
+    (*     Some ((s,t), Rval (Litv (IntLit (Z.of_nat (List.length ws))))) *)
+    (*   | _ => None *)
+    (*   end *)
+    (* | Aupdate, [Loc lnum; Litv (IntLit i); v] => *)
+    (*   match store_lookup lnum s with *)
+    (*   | Some (Varray vs') => *)
+    (*     if (Z_lt_dec i 0)%Z then (* LATER: use a wrapper function for this kind of test *) *)
+    (*       Some ((s,t), Rerr (Rraise sub_exn_v)) *)
+    (*     else *)
+    (*       let n := Z.to_nat i in *)
+    (*       if Nat.leb (List.length vs') n *)
+    (*       then Some ((s,t), Rerr (Rraise sub_exn_v)) *)
+    (*       else *)
+    (*         match store_assign lnum (Varray (update n v vs')) s with *)
+    (*         | None => None *)
+    (*         | Some s' => Some ((s',t), Rval (Conv None [])) *)
+    (*         end *)
+    (*   | _ => None *)
+    (*   end *)
+    (* | ConfigGC, [Litv (IntLit i); Litv (IntLit j)] => *)
+    (*   Some ((s,t), Rval (Conv None [])) *)
+    (* | FFI n, [Litv(StrLit conf); Loc lnum] => *)
+    (*   match store_lookup lnum s with *)
+    (*   | Some (W8array ws) => *)
+    (*     match call_FFI t n (List.map (fun c' => nat_to_word 8 (nat_of_ascii c')) *)
+    (*                                  (string_to_list_char conf)) ws with *)
+    (*     | Ffi_return _ t' ws' => *)
+    (*       match store_assign lnum (W8array ws') s with *)
+    (*       | Some s' => Some ((s', t'), Rval (Conv None [])) *)
+    (*       | None => None *)
+    (*       end *)
+    (*     | Ffi_final _ outcome => *)
+    (*       Some ((s, t), Rerr (Rabort (Rffi_error outcome))) *)
+    (*     end *)
+    (*   | _ => None *)
+    (*   end *)
     | _, _ => None
     end
   end.
@@ -509,121 +509,646 @@ Definition list_result {A B : Type} (res : result A B) : result (list A) B :=
   | Rerr e => Rerr e
   end.
 
-Fixpoint evaluate (fuel : nat) {ffi' : Type} (st : state ffi') (env : sem_env val)
-         (es : list exp) : state ffi' * result (list val) val :=
-  match fuel with
-  | O => (st, Rerr (Rabort Rtimeout_error))
-  | S fuel' =>
-    let fix evaluate_match (st : state ffi') (env : sem_env val) (v' : val)
-            (pes : list (pat * exp)) (err_v : val) : state ffi' * result (list val) val :=
-        match pes with
-        | [] => (st, Rerr (Rraise err_v))
-        | (p,e)::pes' => if NoDuplicates_dec string_dec (pat_bindings p)
-                       then match pmatch (sec env) (refs st) p v' [] with
-                            | Match env_v' => evaluate fuel' st {| sev := nsAppend (alist_to_ns env_v') (sev env);
-                                                                  sec := (sec env) |} [e]
-                            | No_match => evaluate_match st env v' pes' err_v
-                            | Match_type_error => (st, Rerr (Rabort Rtype_error))
-                            end
-                       else (st, Rerr (Rabort Rtype_error))
-        end
-    in
+(* An attempt to use lexicographical induction as the termination condition *)
 
-    let fix evaluate_single_exp (st : state ffi') (env : sem_env val) (ex : exp)
-        : state ffi' * result (list val) val :=
-        match ex with
-        | ELit l => (st, Rval [Litv l])
-        | ERaise e => match evaluate_single_exp st env e with
-                     | (st', Rval (v'::vs')) => (st', Rerr (Rraise v'))
-                     | res => res
-                     end
-        | EHandle e pes => match (evaluate_single_exp st env e) with
-                          | (st', Rerr (Rraise v')) => evaluate_match st' env v' pes v'
-                          | res => res
-                          end
-        | ECon cn es' => if do_con_check (sec env) cn (length es')
-                        then match evaluate fuel' st env (rev es') with
-                             | (st', Rval vs) => match build_conv (sec env) cn (rev vs) with
-                                                | Some v' => (st', Rval [v'])
-                                                | None => (st', Rerr (Rabort Rtype_error))
-                                                end
-                             | res => res
-                             end
-                        else (st, Rerr (Rabort Rtype_error))
-        | EVar n => match nsLookup ident_string_dec n (sev env) with
-                   | Some v' => (st, Rval [v'])
-                   | None => (st, Rerr (Rabort Rtype_error))
-                   end
-        | EFun x e => (st, Rval [Closure env x e])
-
-        | EApp op es => match (evaluate fuel' st env (rev es)) with
-                       | (st', Rval vs) => if op_eq_dec op Opapp
-                                          then match do_opapp (rev vs) with
-                                               | Some (env', e) => evaluate fuel' st' env' [e]
-                                               | None => (st', Rerr (Rabort Rtype_error))
-                                               end
-                                          else match do_app _ (refs st', ffi st') op (rev vs) with
-                                               | Some ((refs, ffi), r) => ({| refs := refs;
-                                                                             ffi  := ffi;
-                                                                             clock := clock st';
-                                                                             next_type_stamp := next_type_stamp st' ;
-                                                                             next_exn_stamp := next_exn_stamp st'
-                                                                          |},
-                                                                          list_result r)
-                                               | None => (st', Rerr (Rabort Rtype_error))
-                                               end
-                       | res => res
-                       end
-
-        | ELog lop e1 e2 => match (evaluate fuel' st env [e1]) with
-                           | (st', Rval (v1::vs1)) => match do_log lop v1 e2 with
-                                                    | Some (Exp e) => evaluate fuel' st' env [e]
-                                                    | Some (Val v') => (st', Rval [v'])
-                                                    | None => (st', Rerr (Rabort Rtype_error))
-                                                    end
-                           | res => res
-                           end
-
-        | EIf e1 e2 e3 => match (evaluate fuel' st env [e1]) with
-                         | (st', Rval (v'::vs')) => match do_if v' e2 e3 with
-                                                  | Some e => evaluate fuel' st' env [e]
-                                                  | None => (st', Rerr (Rabort Rtype_error))
-                                                  end
-                         | res => res
-                         end
-
-        | EMat e pes => match (evaluate fuel' st env [e]) with
-                       | (st', Rval (v'::vs')) => evaluate_match st' env v' pes bind_exn_v
-                       | res => res
-                       end
-
-        | ELet xo e1 e2 => match (evaluate fuel' st env [e1]) with
-                          | (st', Rval (v'::vs')) => evaluate fuel' st'
-                                                            {| sev := nsOptBind xo v' (sev env); sec := (sec env) |} [e2]
-                          | res => res
-                          end
-
-        | ELetrec funs e =>  if NoDuplicates_dec (pair_eq_dec _ _ (pair_eq_dec _ _ string_dec string_dec) exp_eq_dec) funs
-                            then evaluate fuel' st {| sev := build_rec_env funs env (sev env); sec := (sec env) |} [e]
-                            else (st, Rerr (Rabort Rtype_error))
-
-        | ETannot e t => evaluate fuel' st env [e]
-        | ELannot e l => evaluate fuel' st env [e]
-        end
-    in
-
-    match es with
-    | [] => (st, Rval [])
-    | e'::es' => match evaluate_single_exp st env e' with
-               | (st', Rval (v'::vs')) =>
-                 match evaluate fuel' st' env es' with
-                 | (st'', Rval vs'') => (st'', Rval (v'::vs''))
-                 | res => res
-                 end
-               | res => res
-               end
-    end
+Fixpoint size_exp (e : exp) : nat :=
+  let fix size_exps (es : list exp) :=
+      match es with
+      | [] => 0
+      | e'::es' => size_exp e' + size_exps es'
+      end
+  in
+  let fix size_pes (pes : list (pat * exp)) :=
+      match pes with
+      | [] => 0
+      | (_,e)::pes' => size_exp e + size_pes pes'
+      end
+  in
+  match e with
+  (* | ELit _  *)| EVar _ => 1
+  | EMat e' pes => 1 + size_exp e' + size_pes pes
+  | EFun _ e'    (* | ERaise e' *)
+  (* | EHandle e' _ *)
+  (* | ELetrec _ e' | ETannot e' _ *)
+  | ELannot e' _ => 1 + size_exp e'
+  | ECon _ es | EApp _ es => 1 + size_exps es
+  (* | ELet _ e' e'' | ELog _ e' e'' => 1 + size_exp e' + size_exp e'' *)
+  (* | EIf  e' e'' e''' => 1 + size_exp e' + size_exp e'' + size_exp e''' *)
   end.
+
+Fixpoint size_exps (es : list exp) : nat :=
+  match es with
+  | [] => O
+  | e::es' => size_exp e + size_exps es'
+  end.
+
+Fixpoint size_pes (pes : list (pat * exp)) :=
+  match pes with
+  | [] => 0
+  | (_,e)::pes' => size_exp e + size_pes pes'
+  end.
+
+Theorem size_exps_app : forall (es es' : list exp), size_exps (es ++ es') = size_exps es + size_exps es'.
+Proof.
+  induction es.
+  - reflexivity.
+  - intro es'.
+    simpl. rewrite IHes.
+    omega.
+Qed.
+
+Theorem size_exps_rev : forall (es : list exp), size_exps (rev es) = size_exps es.
+Proof.
+  induction es.
+  - reflexivity.
+  - simpl. rewrite size_exps_app.
+    rewrite IHes. simpl. omega.
+Qed.
+
+Inductive fuel_size_rel : nat * list exp -> nat * list exp -> Prop :=
+| fuel_eq : forall (f : nat) (es es' : list exp), size_exps es < size_exps es' -> fuel_size_rel (f, es) (f, es')
+| fuel_less : forall (f f' : nat) (es es' : list exp), f < f' -> fuel_size_rel (f, es) (f', es').
+
+Definition fuel_size_rel_alt (p0 p1 : nat * list exp) : Prop :=
+  let (n0,es0) := p0 in
+  let (n1,es1) := p1 in
+  n0 < n1 \/ n0 = n1 /\ size_exps es0 < size_exps es1.
+
+Require Import Coq.Init.Wf.
+Require Import Omega.
+Require Program.
+
+Definition Rfuel (f f' : nat) := f < f'.
+
+Definition lex_exps (f : nat) := list exp.
+Definition Rsize (f : nat) (es es' : lex_exps f) := size_exps (es) < size_exps es'.
+
+Theorem Rfuel_wf : well_founded Rfuel.
+Proof.
+  red. induction a.
+  - constructor. intros y H.
+    inv H.
+  - constructor.
+    constructor.
+    intros y0 H0.
+    inv IHa.
+    apply H1.
+    unfold Rfuel in *.
+    omega.
+Qed.
+
+Lemma Rsize_wf' : forall f len es, size_exps es <= len -> Acc (Rsize f) es.
+  intros f len.
+  induction len; intros; constructor; intros.
+  - unfold Rsize in *.
+    omega.
+  - apply IHlen.
+    unfold Rsize in *.
+    omega.
+Qed.
+
+Theorem Rsize_wf : forall f, well_founded (Rsize f).
+Proof.
+  red.
+  induction a; constructor; intros.
+  - inv H.
+  - apply Rsize_wf' with (size_exps (a::a0)).
+    unfold Rsize in *.
+    omega.
+Qed.
+
+Require Import Coq.Wellfounded.Lexicographic_Product.
+Require Import Relation_Operators.
+
+Definition lex_f_s := lexprod nat lex_exps Rfuel Rsize.
+Definition lex_f_s_wf := (wf_lexprod nat lex_exps Rfuel Rsize Rfuel_wf Rsize_wf).
+
+Theorem fuckthat : forall (x : pat * exp) (l' l : list (pat * exp)), size_pes (x::l') <= size_pes l -> size_pes l' <= size_pes l.
+Proof.
+  intros [p e] l' l H.
+  simpl in *.
+  omega.
+Defined.
+
+Lemma size_exp_at_least_S : (forall x, 1 <= size_exp x).
+Proof.
+  destruct x; simpl; omega.
+Defined.
+
+Theorem fuel_size_rel_wf' : forall n m f es, f = n /\ size_exps es <= m \/ f < n  -> Acc fuel_size_rel (f, es).
+Proof.
+  induction n.
+  - induction m.
+    + constructor.
+      inv H.
+      * inv H0.
+        intros.
+        inv H.
+        omega.
+        omega.
+      * inv H0.
+    + constructor.
+      intros.
+      inv H.
+      inv H1.
+      inv H0.
+      apply IHm.
+      left; split; omega.
+      omega.
+      omega.
+  - induction m.
+    + constructor.
+      intros; destruct y.
+      inv H0.
+      inv H.
+      inv H0.
+      omega.
+      inv H0.
+      apply IHn with (size_exps es).
+      left; omega.
+      apply IHn with (size_exps es).
+      right; omega.
+      inv H.
+      inv H0.
+      apply IHn with (size_exps l).
+      inv H2.
+      left; omega.
+      right; omega.
+      apply IHn with n0.
+      right; omega.
+    + constructor.
+      intros; destruct y.
+      inv H.
+      inv H1.
+      inv H0.
+      apply IHm.
+      left; omega.
+      apply IHm.
+      right; omega.
+      inv H0.
+      apply IHm.
+      right; omega.
+      apply IHm.
+      right; omega.
+Defined.
+
+Theorem fuel_size_rel_wf : well_founded fuel_size_rel.
+Proof.
+  unfold well_founded.
+  destruct a.
+  induction n; constructor; intros.
+  inv H.
+  apply fuel_size_rel_wf' with (n := 0) (m := size_exps l).
+  left; omega.
+  inv H2.
+  inv H.
+  apply fuel_size_rel_wf' with (n := S n) (m := size_exps l).
+  left; omega.
+  apply fuel_size_rel_wf' with f (size_exps es).
+  left; omega.
+Defined.
+
+(*----------------------------------------------------------------------------*)
+(*------------- EQUATIONS VERSION ------------------------------------------- *)
+(*----------------------------------------------------------------------------*)
+Require Import Equations.Equations.
+
+Instance FSRWellFounded : WellFounded fuel_size_rel.
+apply fuel_size_rel_wf.
+Qed.
+
+Equations evaluate {ffi' : Type} (es : list exp) (fuel : nat) (st : state ffi') (env : sem_env val)
+  : state ffi' * result (list val) val by wf (fuel, es) fuel_size_rel := {
+  evaluate [] _ st _ => (st, Rval []);
+  evaluate (e1::e2::es') fuel st env =>
+    match evaluate [e1] fuel st env with
+    | (st', Rval vs) => (* This differs from lem semantics*)
+      match evaluate (e2::es') fuel st' env with
+      | (st'', Rval vs'') =>
+        match vs with
+        | [] => (st'', Rval vs'') (* This should never happen *)
+        | v::vs' => (st'', Rval (v::vs''))
+        end
+      | res => res
+      end
+    | res => res
+    end;
+  evaluate [EVar n] _ st env => match nsLookup ident_string_dec n (sev env) with
+                     | Some v' => (st, Rval [v'])
+                     | None => (st, Rerr (Rabort Rtype_error))
+                     end;
+  evaluate [ECon cn es'] fuel st env =>
+       if do_con_check (sec env) cn (length es')
+       then match evaluate (rev es') fuel st env with
+            | (st', Rval vs) => match build_conv (sec env) cn (rev vs) with
+                               | Some v' => (st', Rval [v'])
+                               | None => (st', Rerr (Rabort Rtype_error))
+                               end
+            | res => res
+            end
+       else (st, Rerr (Rabort Rtype_error));
+  evaluate [EFun x e] _ st _=> (st, Rval [Closure env x e]);
+  evaluate [EApp op es] 0 st env => (st, Rerr (Rabort Rtimeout_error));
+  evaluate [EApp op es] (S fuel') st env =>
+        match (evaluate (rev es) fuel' st env) with
+        | (st', Rval vs) => if op_eq_dec op Opapp
+                           then match do_opapp (rev vs) with
+                                | Some (env', e) => evaluate [e] fuel' st' env'
+                                | None => (st', Rerr (Rabort Rtype_error))
+                                end
+                           else match do_app _ (refs st', ffi st') op (rev vs) with
+                                | Some ((refs, ffi), r) => ({| refs := refs;
+                                                              ffi  := ffi;
+                                                              clock := clock st';
+                                                              next_type_stamp := next_type_stamp st' ;
+                                                              next_exn_stamp := next_exn_stamp st'
+                                                           |},
+                                                           list_result r)
+                                | None => (st', Rerr (Rabort Rtype_error))
+                                end
+        | res => res
+        end;
+  evaluate [EMat e pes] _ st env =>
+      match (evaluate [e] fuel st env) with
+      | (st', Rval (v'::vs')) =>
+        (fix evaluate_match (pes0 : list (pat * exp)) err_v (H : size_pes pes0 <= size_pes pes) :=
+           match pes0 as y return pes0 = y -> state ffi' * result (list val) val with
+           | [] => fun H0 => (st, Rerr (Rraise err_v))
+           | (p,e)::pes0' => fun H0 =>
+                         if NoDuplicates_dec string_dec (pat_bindings p)
+                         then (match pmatch (sec env) (refs st) p v' [] with
+                               | Match env_v' =>
+                                 evaluate [e] fuel st
+                                   {| sev := nsAppend (alist_to_ns env_v') (sev env);
+                                      sec := (sec env) |}
+                               | No_match => evaluate_match pes0' err_v
+                                              (fuckthat (p,e) pes0' pes (eq_ind pes0 (fun p => size_pes p <= size_pes pes) H ((p,e)::pes0') H0))
+                               | Match_type_error => (st, Rerr (Rabort Rtype_error))
+                               end)
+                         else (st, Rerr (Rabort Rtype_error))
+           end (eq_refl)) pes bind_exn_v (le_n (size_pes pes))
+      | res => res
+      end;
+  evaluate [ELannot e l] fuel st env => evaluate [e] fuel st env}.
+Obligation 1.
+constructor.
+rewrite size_exps_rev.
+simpl. fold size_exps.
+omega.
+Qed.
+Obligation 2.
+constructor; simpl; omega.
+Qed.
+Obligation 3.
+constructor; simpl; omega.
+Qed.
+Obligation 4.
+(* specialize (size_exp_at_least_S e2). *)
+constructor; simpl; omega.
+Qed.
+Obligation 5.
+specialize (size_exp_at_least_S e0).
+constructor; simpl. fold size_pes. omega.
+Qed.
+Obligation 6.
+constructor; simpl; omega.
+Qed.
+Obligation 7.
+specialize (size_exp_at_least_S e2).
+constructor; simpl; omega.
+Qed.
+Obligation 8.
+specialize (size_exp_at_least_S e1).
+constructor; simpl; omega.
+Qed.
+Obligations.
+
+(*----------------------------------------------------------------------------*)
+(*------------- LEXICOGRAPHIC VERSION --------------------------------------- *)
+(*----------------------------------------------------------------------------*)
+
+(* Program Fixpoint evaluate {ffi' : Type} (es : list exp) (fuel : nat) (st : state ffi') (env : sem_env val) *)
+(*         {measure (fuel,es) fuel_size_rel }  : state ffi' * result (list val) val := *)
+(*   match es with *)
+(*   | [] => (st, Rval []) *)
+(*   | [EVar n] => match nsLookup ident_string_dec n (sev env) with *)
+(*                | Some v' => (st, Rval [v']) *)
+(*                | None => (st, Rerr (Rabort Rtype_error)) *)
+(*                end *)
+(*   | [EFun x e] => (st, Rval [Closure env x e]) *)
+(*   | [ECon cn es'] => if do_con_check (sec env) cn (length es') *)
+(*                     then match evaluate (rev es') fuel st env with *)
+(*                          | (st', Rval vs) => match build_conv (sec env) cn (rev vs) with *)
+(*                                             | Some v' => (st', Rval [v']) *)
+(*                                             | None => (st', Rerr (Rabort Rtype_error)) *)
+(*                                             end *)
+(*                          | res => res *)
+(*                          end *)
+(*                     else (st, Rerr (Rabort Rtype_error)) *)
+
+(*   | [EApp op es] => match fuel with *)
+(*                    | O => (st, Rerr (Rabort Rtimeout_error)) *)
+(*                    | S fuel' => *)
+(*                      match (evaluate (rev es) fuel' st env) with *)
+(*                      | (st', Rval vs) => if op_eq_dec op Opapp *)
+(*                                         then match do_opapp (rev vs) with *)
+(*                                              | Some (env', e) => evaluate [e] fuel' st' env' *)
+(*                                              | None => (st', Rerr (Rabort Rtype_error)) *)
+(*                                              end *)
+(*                                         else match do_app _ (refs st', ffi st') op (rev vs) with *)
+(*                                              | Some ((refs, ffi), r) => ({| refs := refs; *)
+(*                                                                            ffi  := ffi; *)
+(*                                                                            clock := clock st'; *)
+(*                                                                            next_type_stamp := next_type_stamp st' ; *)
+(*                                                                            next_exn_stamp := next_exn_stamp st' *)
+(*                                                                         |}, *)
+(*                                                                         list_result r) *)
+(*                                              | None => (st', Rerr (Rabort Rtype_error)) *)
+(*                                              end *)
+(*                      | res => res *)
+(*                      end *)
+(*                    end *)
+
+(*   | [EMat e pes] => match (evaluate [e] fuel st env) with *)
+(*                    | (st', Rval (v'::vs')) => *)
+(*                      (fix evaluate_match (pes0 : list (pat * exp)) (err_v : val) (H : size_pes pes0 <= size_pes pes) *)
+(*                       : state ffi' * result (list val) val := *)
+(*                         match pes0 as y with *)
+(*                         | [] => (st, Rerr (Rraise err_v)) *)
+(*                         | (p,e0)::pes0' => *)
+(*                           if NoDuplicates_dec string_dec (pat_bindings p) *)
+(*                           then (match pmatch (sec env) (refs st) p v' [] with *)
+(*                                | Match env_v' => *)
+(*                                  evaluate [e0] fuel st *)
+(*                                           {| sev := nsAppend (alist_to_ns env_v') (sev env); *)
+(*                                              sec := (sec env) |} *)
+(*                                | No_match => evaluate_match pes0' err_v (fuckthat (p,e0) pes0' pes H) *)
+(*                                | Match_type_error => (st, Rerr (Rabort Rtype_error)) *)
+(*                                 end) *)
+(*                           else (st, Rerr (Rabort Rtype_error)) *)
+(*                         end) *)
+(*                        pes bind_exn_v (le_n (size_pes pes)) *)
+(*                    | res => res *)
+(*     end *)
+(*   (* end *) *)
+
+(*   | [ELannot e l] => evaluate [e] fuel st env *)
+
+(*   | e::es' => match evaluate [e] fuel st env with *)
+(*             | (st', Rval vs) => (* This differs from lem semantics*) *)
+(*               match evaluate es' fuel st' env with *)
+(*               | (st'', Rval vs'') => *)
+(*                 match vs with *)
+(*                 | [] => (st'', Rval vs'') (* This should never happen *) *)
+(*                 | v::vs' => (st'', Rval (v::vs'')) *)
+(*                 end *)
+(*               | res => res *)
+(*               end *)
+(*             | res => res *)
+(*             end *)
+(*   end. *)
+(* Obligation 1. *)
+(* constructor. *)
+(* rewrite size_exps_rev. *)
+(* induction es'. *)
+(* - simpl; omega. *)
+(* - simpl. *)
+(*   rewrite <- plus_n_O. *)
+(*   fold size_exps. *)
+(*   omega. *)
+(* Defined. *)
+(* Obligation 3. *)
+(* constructor. *)
+(* omega. *)
+(* Defined. *)
+(* Obligation 4. *)
+(* constructor; omega. *)
+(* Defined. *)
+(* Obligation 6. *)
+(* constructor. *)
+(* simpl; omega. *)
+(* Defined. *)
+(* Obligation 7. *)
+(* specialize (size_exp_at_least_S e0). *)
+(* inv H; constructor; *)
+(* simpl in *; fold size_pes; omega. *)
+(* Defined. *)
+(* Obligation 11. *)
+(* constructor; simpl. *)
+(* omega. *)
+(* Defined. *)
+(* Obligation 12. *)
+(* constructor. *)
+(* destruct es'. destruct e; congruence. *)
+(* simpl. *)
+(* specialize (size_exp_at_least_S e). *)
+(* specialize (size_exp_at_least_S e0). *)
+(* omega. *)
+(* Defined. *)
+(* Obligation 13. *)
+(* destruct es'. destruct e; congruence. *)
+(* specialize (size_exp_at_least_S e). *)
+(* specialize (size_exp_at_least_S e0). *)
+(* constructor; simpl; omega. *)
+(* Defined. *)
+(* Obligation 16. *)
+(* repeat (split; try (congruence)). *)
+(* Defined. *)
+(* Obligation 17. *)
+(* repeat (split; try (congruence)). *)
+(* Defined. *)
+(* Obligation 18. *)
+(* repeat (split; try (congruence)). *)
+(* Defined. *)
+(* Obligation 19. *)
+(* repeat (split; try (congruence)). *)
+(* Defined. *)
+(* Obligation 20. *)
+(* repeat (split; try (congruence)). *)
+(* Defined. *)
+(* Obligation 21. *)
+(* repeat (split; try (congruence)). *)
+(* Defined. *)
+(* Obligation 22. *)
+(* (* HOW DO I ACTUALLY SOLVE THIS. *) *)
+(* auto using fuel_size_rel_wf. *)
+(* Defined. *)
+
+(*----------------------------------------------------------------------------*)
+(*------------- FUEL TERMINATION VERSION -------------------------------------*)
+(*----------------------------------------------------------------------------*)
+
+(* Fixpoint evaluate {ffi' : Type} (es : list exp) (fuel : nat)  (st : state ffi') (env : sem_env val) *)
+(*          : state ffi' * result (list val) val := *)
+(*     match es with *)
+(*     | [] => (st, Rval []) *)
+(*     | [EVar n] => match nsLookup ident_string_dec n (sev env) with *)
+(*                  | Some v' => (st, Rval [v']) *)
+(*                  | None => (st, Rerr (Rabort Rtype_error)) *)
+(*                  end *)
+(*     | [EFun x e] => (st, Rval [Closure env x e]) *)
+(*     | [ECon cn es'] => if do_con_check (sec env) cn (length es') *)
+(*                       then match fuel with *)
+(*                            | O => (st, Rerr (Rabort Rtimeout_error)) *)
+(*                            | S fuel' => *)
+(*                              match evaluate (rev es') fuel' st env with *)
+(*                              | (st', Rval vs) => match build_conv (sec env) cn (rev vs) with *)
+(*                                                 | Some v' => (st', Rval [v']) *)
+(*                                                 | None => (st', Rerr (Rabort Rtype_error)) *)
+(*                                                 end *)
+(*                              | res => res *)
+(*                              end *)
+(*                            end *)
+(*                       else (st, Rerr (Rabort Rtype_error)) *)
+
+(*     | [EApp op es] => match fuel with *)
+(*                      | O => (st, Rerr (Rabort Rtimeout_error)) *)
+(*                      | S fuel' => *)
+(*                        match (evaluate (rev es) fuel' st env) with *)
+(*                        | (st', Rval vs) => if op_eq_dec op Opapp *)
+(*                                           then match do_opapp (rev vs) with *)
+(*                                                | Some (env', e) => evaluate [e] fuel' st' env' *)
+(*                                                | None => (st', Rerr (Rabort Rtype_error)) *)
+(*                                                end *)
+(*                                           else match do_app _ (refs st', ffi st') op (rev vs) with *)
+(*                                                | Some ((refs, ffi), r) => ({| refs := refs; *)
+(*                                                                              ffi  := ffi; *)
+(*                                                                              clock := clock st'; *)
+(*                                                                              next_type_stamp := next_type_stamp st' ; *)
+(*                                                                              next_exn_stamp := next_exn_stamp st' *)
+(*                                                                           |}, *)
+(*                                                                           list_result r) *)
+(*                                                | None => (st', Rerr (Rabort Rtype_error)) *)
+(*                                                end *)
+(*                        | res => res *)
+(*                        end *)
+(*                      end *)
+
+(*     | [EMat e pes] => match fuel with *)
+(*                      | O => (st, Rerr (Rabort Rtimeout_error)) *)
+(*                      | S fuel' => *)
+(*                        match (evaluate [e] fuel' st env) with *)
+(*                        | (st', Rval (v'::vs')) => *)
+(*                          (fix evaluate_match (st : state ffi') (env : sem_env val) (v' : val) *)
+(*                               (pes : list (pat * exp)) (err_v : val) : state ffi' * result (list val) val := *)
+(*                             match pes with *)
+(*                             | [] => (st, Rerr (Rraise err_v)) *)
+(*                             | (p,e)::pes' => *)
+(*                               if NoDuplicates_dec string_dec (pat_bindings p) *)
+(*                               then match pmatch (sec env) (refs st) p v' [] with *)
+(*                                    | Match env_v' => evaluate [e] fuel' st {| sev := nsAppend (alist_to_ns env_v') (sev env); *)
+(*                                                                          sec := (sec env) |} *)
+(*                                    | No_match => evaluate_match st env v' pes' err_v *)
+(*                                    | Match_type_error => (st, Rerr (Rabort Rtype_error)) *)
+(*                                    end *)
+(*                               else (st, Rerr (Rabort Rtype_error)) *)
+(*                             end) *)
+(*                            st' env v' pes bind_exn_v *)
+(*                        | res => res *)
+(*                        end *)
+(*                      end *)
+
+(*     | [ELannot e l] => match fuel with *)
+(*                       | O => (st, Rerr (Rabort Rtimeout_error)) *)
+(*                       | S fuel' => evaluate [e] fuel' st env *)
+(*                       end *)
+
+(*     | e::es' => match fuel with *)
+(*               | O => (st, Rerr (Rabort Rtimeout_error)) *)
+(*               | S fuel' => *)
+(*                 match evaluate [e] fuel' st env with *)
+(*                 | (st', Rval vs) => (* This differs from lem semantics*) *)
+(*                   match evaluate es' fuel' st' env with *)
+(*                   | (st'', Rval vs'') => *)
+(*                     match vs with *)
+(*                     | [] => (st'', Rval vs'') (* This should never happen *) *)
+(*                     | v::vs' => (st'', Rval (v::vs'')) *)
+(*                     end *)
+(*                   | res => res *)
+(*                   end *)
+(*                 | res => res *)
+(*                 end *)
+(*               end *)
+(*     end. *)
+
+(* 'Old' evaluate *)
+(* Fixpoint evaluate (fuel : nat) {ffi' : Type} (st : state ffi') (env : sem_env val) *)
+(*          (es : list exp) : state ffi' * result (list val) val := *)
+(*   match fuel with *)
+(*   | O => (st, Rerr (Rabort Rtimeout_error)) *)
+(*   | S fuel' => *)
+(*     match es with *)
+(*     | [] => (st, Rval []) *)
+(*     | [EVar n] => match nsLookup ident_string_dec n (sev env) with *)
+(*                  | Some v' => (st, Rval [v']) *)
+(*                  | None => (st, Rerr (Rabort Rtype_error)) *)
+(*                  end *)
+(*     | [EFun x e] => (st, Rval [Closure env x e]) *)
+(*     | [ECon cn es'] => if do_con_check (sec env) cn (length es') *)
+(*                       then match evaluate fuel' st env (rev es') with *)
+(*                            | (st', Rval vs) => match build_conv (sec env) cn (rev vs) with *)
+(*                                               | Some v' => (st', Rval [v']) *)
+(*                                               | None => (st', Rerr (Rabort Rtype_error)) *)
+(*                                               end *)
+(*                            | res => res *)
+(*                            end *)
+(*                       else (st, Rerr (Rabort Rtype_error)) *)
+
+(*     | [EApp op es] => match (evaluate fuel' st env (rev es)) with *)
+(*                      | (st', Rval vs) => if op_eq_dec op Opapp *)
+(*                                         then match do_opapp (rev vs) with *)
+(*                                              | Some (env', e) => evaluate fuel' st' env' [e] *)
+(*                                              | None => (st', Rerr (Rabort Rtype_error)) *)
+(*                                              end *)
+(*                                         else match do_app _ (refs st', ffi st') op (rev vs) with *)
+(*                                              | Some ((refs, ffi), r) => ({| refs := refs; *)
+(*                                                                            ffi  := ffi; *)
+(*                                                                            clock := clock st'; *)
+(*                                                                            next_type_stamp := next_type_stamp st' ; *)
+(*                                                                            next_exn_stamp := next_exn_stamp st' *)
+(*                                                                         |}, *)
+(*                                                                         list_result r) *)
+(*                                              | None => (st', Rerr (Rabort Rtype_error)) *)
+(*                                              end *)
+(*                      | res => res *)
+(*                      end *)
+
+(*     | [EMat e pes] => match (evaluate fuel' st env [e]) with *)
+(*                      | (st', Rval (v'::vs')) => *)
+(*                        (fix evaluate_match (st : state ffi') (env : sem_env val) (v' : val) *)
+(*                             (pes : list (pat * exp)) (err_v : val) : state ffi' * result (list val) val := *)
+(*                           match pes with *)
+(*                           | [] => (st, Rerr (Rraise err_v)) *)
+(*                           | (p,e)::pes' => *)
+(*                             if NoDuplicates_dec string_dec (pat_bindings p) *)
+(*                             then match pmatch (sec env) (refs st) p v' [] with *)
+(*                                  | Match env_v' => evaluate fuel' st {| sev := nsAppend (alist_to_ns env_v') (sev env); *)
+(*                                                                        sec := (sec env) |} [e] *)
+(*                                  | No_match => evaluate_match st env v' pes' err_v *)
+(*                                  | Match_type_error => (st, Rerr (Rabort Rtype_error)) *)
+(*                                  end *)
+(*                             else (st, Rerr (Rabort Rtype_error)) *)
+(*                           end) *)
+(*                          st' env v' pes bind_exn_v *)
+(*                      | res => res *)
+(*                      end *)
+
+(*     | [ELannot e l] => evaluate fuel' st env [e] *)
+
+(*     | e::es' => match evaluate fuel' st env [e] with *)
+(*               | (st', Rval vs) => (* This differs from lem semantics*) *)
+(*                 match evaluate fuel' st' env es' with *)
+(*                 | (st'', Rval vs'') => *)
+(*                   match vs with *)
+(*                   | [] => (st'', Rval vs'') (* This should never happen *) *)
+(*                   | v::vs' => (st'', Rval (v::vs'')) *)
+(*                   end *)
+(*                 | res => res *)
+(*                 end *)
+(*               | res => res *)
+(*               end *)
+(*     end *)
+(*   end. *)
 
 Fixpoint identity_to_string (i : ident modN varN) : string :=
   match i with
@@ -654,15 +1179,15 @@ Fixpoint evaluate_opt {ffi' : Type} (st : state ffi') (env : sem_env val)
     let fix evaluate_single_exp (st : state ffi') (env : sem_env val) (ex : exp)
         : state ffi' * result (list val) val :=
         match ex with
-        | ELit l => (st, Rval [Litv l])
-        | ERaise e => match evaluate_single_exp st env e with
-                     | (st', Rval (v'::vs')) => (st', Rerr (Rraise v'))
-                     | res => res
-                     end
-        | EHandle e pes => match (evaluate_single_exp st env e) with
-                          | (st', Rerr (Rraise v')) => evaluate_match st' env v' pes v'
-                          | res => res
-                          end
+        (* | ELit l => (st, Rval [Litv l]) *)
+        (* | ERaise e => match evaluate_single_exp st env e with *)
+        (*              | (st', Rval (v'::vs')) => (st', Rerr (Rraise v')) *)
+        (*              | res => res *)
+        (*              end *)
+        (* | EHandle e pes => match (evaluate_single_exp st env e) with *)
+        (*                   | (st', Rerr (Rraise v')) => evaluate_match st' env v' pes v' *)
+        (*                   | res => res *)
+        (*                   end *)
         | ECon cn es' => if do_con_check (sec env) cn (length es')
                         then match (evaluate_opt st env (rev es') fuel') with
                              | (st', Rval vs) => match build_conv (sec env) cn (rev vs) with
@@ -698,39 +1223,39 @@ Fixpoint evaluate_opt {ffi' : Type} (st : state ffi') (env : sem_env val)
                        | res => res
                        end
 
-        | ELog lop e1 e2 => match (evaluate_opt st env [e1] fuel') with
-                           | (st', Rval (v1::vs1)) => match do_log lop v1 e2 with
-                                                    | Some (Exp e) => (evaluate_opt st' env [e] fuel')
-                                                    | Some (Val v') => (st', Rval [v'])
-                                                    | None => (st', Rerr (Rabort Rtype_error))
-                                                    end
-                           | res => res
-                           end
+        (* | ELog lop e1 e2 => match (evaluate_opt st env [e1] fuel') with *)
+        (*                    | (st', Rval (v1::vs1)) => match do_log lop v1 e2 with *)
+        (*                                             | Some (Exp e) => (evaluate_opt st' env [e] fuel') *)
+        (*                                             | Some (Val v') => (st', Rval [v']) *)
+        (*                                             | None => (st', Rerr (Rabort Rtype_error)) *)
+        (*                                             end *)
+        (*                    | res => res *)
+        (*                    end *)
 
-        | EIf e1 e2 e3 => match (evaluate_opt st env [e1] fuel') with
-                         | (st', Rval (v'::vs')) => match do_if v' e2 e3 with
-                                                  | Some e => (evaluate_opt st' env [e] fuel')
-                                                  | None => (st', Rerr (Rabort Rtype_error))
-                                                  end
-                         | res => res
-                         end
+        (* | EIf e1 e2 e3 => match (evaluate_opt st env [e1] fuel') with *)
+        (*                  | (st', Rval (v'::vs')) => match do_if v' e2 e3 with *)
+        (*                                           | Some e => (evaluate_opt st' env [e] fuel') *)
+        (*                                           | None => (st', Rerr (Rabort Rtype_error)) *)
+        (*                                           end *)
+        (*                  | res => res *)
+        (*                  end *)
 
         | EMat e pes => match (evaluate_opt st env [e] fuel') with
                        | (st', Rval (v'::vs')) => evaluate_match st' env v' pes bind_exn_v
                        | res => res
                        end
 
-        | ELet xo e1 e2 => match (evaluate_opt st env [e1] fuel') with
-                          | (st', Rval (v'::vs')) => (evaluate_opt st'
-                                                                 {| sev := nsOptBind xo v' (sev env); sec := (sec env) |} [e2] fuel')
-                          | res => res
-                          end
+        (* | ELet xo e1 e2 => match (evaluate_opt st env [e1] fuel') with *)
+        (*                   | (st', Rval (v'::vs')) => (evaluate_opt st' *)
+        (*                                                          {| sev := nsOptBind xo v' (sev env); sec := (sec env) |} [e2] fuel') *)
+        (*                   | res => res *)
+        (*                   end *)
 
-        | ELetrec funs e =>  if NoDuplicates_dec (pair_eq_dec _ _ (pair_eq_dec _ _ string_dec string_dec) exp_eq_dec) funs
-                            then (evaluate_opt st {| sev := build_rec_env funs env (sev env); sec := (sec env) |} [e] fuel')
-                            else (st, Rerr (Rabort Rtype_error))
+        (* | ELetrec funs e =>  if NoDuplicates_dec (pair_eq_dec _ _ (pair_eq_dec _ _ string_dec string_dec) exp_eq_dec) funs *)
+        (*                     then (evaluate_opt st {| sev := build_rec_env funs env (sev env); sec := (sec env) |} [e] fuel') *)
+        (*                     else (st, Rerr (Rabort Rtype_error)) *)
 
-        | ETannot e t => (evaluate_opt st env [e] fuel')
+        (* | ETannot e t => (evaluate_opt st env [e] fuel') *)
         | ELannot e l => (evaluate_opt st env [e] fuel')
         end
     in
@@ -748,35 +1273,15 @@ Fixpoint evaluate_opt {ffi' : Type} (st : state ffi') (env : sem_env val)
     end
   end.
 
-Fixpoint size_exp (e : exp) : nat :=
-  let fix size_exps (es : list exp) :=
-      match es with
-      | [] => 0
-      | e'::es => size_exp e' + size_exps es
-      end
-  in
-  match e with
-  | ELit _ | EVar _ => 1
-  | EFun _ e'    | ERaise e'
-  | EHandle e' _ | EMat e' _
-  | ELetrec _ e' | ETannot e' _
-  | ELannot e' _ => 1 + size_exp e'
-  | ECon _ es | EApp _ es => 1 + size_exps es
-  | ELet _ e' e'' | ELog _ e' e'' => 1 + size_exp e' + size_exp e''
-  | EIf  e' e'' e''' => 1 + size_exp e' + size_exp e'' + size_exp e'''
-  end.
-
-Definition size_exps (es : list exp) : nat := fold_left plus (map size_exp es) O.
-
 Fixpoint size_dec (d : dec) : nat :=
   match d with
   | Dlet _ _ _ => 1
   | Dletrec _ _ => 1
   | Dtype _ _ => 1
-  | Dtabbrev _ _ _ _ => 1
-  | Dexn _ _ _ => 1
-  | Dmod _ ds => 1 + fold_left plus (List.map size_dec ds) O
-  | Dlocal lds ds => 1 + fold_left plus (List.map size_dec ds) O + fold_left plus (List.map size_dec lds) O
+  (* | Dtabbrev _ _ _ _ => 1 *)
+  (* | Dexn _ _ _ => 1 *)
+  (* | Dmod _ ds => 1 + fold_left plus (List.map size_dec ds) O *)
+  (* | Dlocal lds ds => 1 + fold_left plus (List.map size_dec ds) O + fold_left plus (List.map size_dec lds) O *)
   end.
 
 Definition size_decs (ds : list dec) : nat := fold_left plus (map size_dec ds) O.
@@ -786,70 +1291,44 @@ Proof.
  destruct d; simpl; omega.
 Qed.
 
-Program Fixpoint evaluate_decs {ffi' : Type} (fuel : nat) (st : state ffi') (env : sem_env val) (decl : list dec) {measure (size_decs decl)}:
-  (state ffi' * result (sem_env val) val) :=
-  let fuel' := fuel in
-  (* match fuel with *)
-  (* | O => (st, Rerr (Rabort Rtimeout_error)) *)
-  (* | S fuel' => *)
-    match decl with
-    | [] => (st, Rval empty_sem_env)
-    | d1::d2::decl' => match evaluate_decs fuel' st env [d1] with
-                    | (st1, Rval env1) =>
-                      match evaluate_decs fuel' st1 (extend_dec_env env1 env) (d2::decl') with
-                      | (st2, r) => (st2, combine_dec_result env1 r)
-                      end
-                    | res => res
-                    end
-
-    | [Dlet locs p e] =>
-      if NoDuplicates_dec string_dec (pat_bindings p)
-      then match evaluate_opt st env [e] fuel with
-           | (st', Rval v) =>
-             (st', match pmatch (sec env) (refs st') p (hd (Litv (StrLit "IF HERE THEN BAD")) v) [] with
-                   | Match new_vals => Rval {| sec := nsEmpty; sev := alist_to_ns new_vals |}
-                   | No_match => Rerr (Rraise bind_exn_v)
-                   | Match_type_error => Rerr (Rabort Rtype_error)
-                   end)
-           | (st', Rerr err) => (st', Rerr err)
-           end
-      else (st, Rerr (Rabort Rtype_error))
-
-    | [Dletrec locs funs] => (st,
-                             if NoDuplicates_dec string_dec (map (fun x => fst (fst x)) funs)
-                             then Rval {| sev := build_rec_env funs env nsEmpty; sec := nsEmpty |}
-                             else Rerr (Rabort Rtype_error))
-
-    | [Dtype locs tds] => if UniqueCtorsInDefs_dec tds
-                         then (state_update_next_type_stamp st (next_type_stamp st + List.length tds),
-                               Rval {| sev := nsEmpty; sec := build_tdefs (next_type_stamp st) tds |})
-                         else (st, Rerr (Rabort Rtype_error))
-    | [Dtabbrev locs tvs tn t] => (st, Rval {| sev := nsEmpty; sec := nsEmpty |})
-    | [Dexn locs cn ts] => (state_update_next_exn_stamp st (next_exn_stamp st + 1),
-                           Rval {| sev := nsEmpty;
-                                   sec := nsSing cn (List.length ts, ExnStamp (next_exn_stamp st)) |})
-    | [Dmod mn ds] => match evaluate_decs fuel' st env ds with
-                     | (st', r) => (st',
-                                   match r with
-                                   | Rval env' => Rval {| sev := nsLift mn (sev env');
-                                                         sec := nsLift mn (sec env') |}
-                                   | Rerr err => Rerr err
-                                   end)
-                     end
-    | [Dlocal lds ds] => match evaluate_decs fuel' st env lds with
-                        | (st1, Rval env1) =>
-                          evaluate_decs fuel' st1 (extend_dec_env env1 env) ds
-                        | res => res
-                        end
-    end.
+Equations evaluate_decs {ffi' : Type} (fuel : nat) (st : state ffi') (env : sem_env val) (decl : list dec)
+  : state ffi' * result (sem_env val) val by wf (size_decs decl) := {
+    evaluate_decs _ st _ [] => (st, Rval empty_sem_env);
+    evaluate_decs fuel st env (d1::d2::decl') =>
+    match evaluate_decs fuel st env [d1] with
+    | (st1, Rval env1) =>
+      match evaluate_decs fuel st1 (extend_dec_env env1 env) (d2::decl') with
+      | (st2, r) => (st2, combine_dec_result env1 r)
+      end
+    | res => res
+    end;
+    evaluate_decs fuel st env [Dlet locs p e] =>
+    if NoDuplicates_dec string_dec (pat_bindings p)
+    then match evaluate_opt st env [e] fuel with
+         | (st', Rval v) =>
+           (st', match pmatch (sec env) (refs st') p (hd (Litv (StrLit "IF HERE THEN BAD")) v) [] with
+                 | Match new_vals => Rval {| sec := nsEmpty; sev := alist_to_ns new_vals |}
+                 | No_match => Rerr (Rraise bind_exn_v)
+                 | Match_type_error => Rerr (Rabort Rtype_error)
+                 end)
+         | (st', Rerr err) => (st', Rerr err)
+         end
+    else (st, Rerr (Rabort Rtype_error));
+    evaluate_decs fuel st env [Dletrec locs funs] =>
+    (st,
+     if NoDuplicates_dec string_dec (map (fun x => fst (fst x)) funs)
+     then Rval {| sev := build_rec_env funs env nsEmpty; sec := nsEmpty |}
+     else Rerr (Rabort Rtype_error));
+    evaluate_decs fuel st env [Dtype locs tds] =>
+    if UniqueCtorsInDefs_dec tds
+    then (state_update_next_type_stamp st (next_type_stamp st + List.length tds),
+          Rval {| sev := nsEmpty; sec := build_tdefs (next_type_stamp st) tds |})
+    else (st, Rerr (Rabort Rtype_error)) }.
 Obligation 1.
 unfold size_decs. simpl.
-
 assert (fold_addition_lt : forall (l : list nat) (n m : nat), n < m -> n < fold_left plus l m).
     (induction l; intros n m H; try (specialize (IHl n (m+a))); simpl; omega).
-
 pose size_dec_min_1 as H.
-
 destruct d1; simpl;
 try (apply fold_addition_lt;
 specialize (size_dec_min_1 d2); omega).
@@ -861,17 +1340,94 @@ induction l; intros m n H.
 simpl; omega.
 simpl. rewrite <- (plus_assoc m n a). rewrite (plus_comm n a). rewrite (plus_assoc m a n).
 apply IHl. omega.
-
 rewrite plus_comm.
 apply fold_addition_lt.
 specialize (size_dec_min_1 d2).
 specialize (size_dec_min_1 d1).
 omega.
 Qed.
-Obligation 5.
-unfold size_decs.
-simpl. omega.
-Qed.
-Obligation 6.
-unfold size_decs. simpl. omega.
-Qed.
+
+(* Program Fixpoint evaluate_decs {ffi' : Type} (fuel : nat) (st : state ffi') (env : sem_env val) (decl : list dec) *)
+(*         {measure (size_decs decl)}: *)
+(*   (state ffi' * result (sem_env val) val) := *)
+(*   let fuel' := fuel in *)
+(*   (* match fuel with *) *)
+(*   (* | O => (st, Rerr (Rabort Rtimeout_error)) *) *)
+(*   (* | S fuel' => *) *)
+(*     match decl with *)
+(*     | [] => (st, Rval empty_sem_env) *)
+(*     | d1::d2::decl' => match evaluate_decs fuel' st env [d1] with *)
+(*                     | (st1, Rval env1) => *)
+(*                       match evaluate_decs fuel' st1 (extend_dec_env env1 env) (d2::decl') with *)
+(*                       | (st2, r) => (st2, combine_dec_result env1 r) *)
+(*                       end *)
+(*                     | res => res *)
+(*                     end *)
+
+(*     | [Dlet locs p e] => *)
+(*       if NoDuplicates_dec string_dec (pat_bindings p) *)
+(*       then match evaluate_opt st env [e] fuel with *)
+(*            | (st', Rval v) => *)
+(*              (st', match pmatch (sec env) (refs st') p (hd (Litv (StrLit "IF HERE THEN BAD")) v) [] with *)
+(*                    | Match new_vals => Rval {| sec := nsEmpty; sev := alist_to_ns new_vals |} *)
+(*                    | No_match => Rerr (Rraise bind_exn_v) *)
+(*                    | Match_type_error => Rerr (Rabort Rtype_error) *)
+(*                    end) *)
+(*            | (st', Rerr err) => (st', Rerr err) *)
+(*            end *)
+(*       else (st, Rerr (Rabort Rtype_error)) *)
+
+(*     | [Dletrec locs funs] => (st, *)
+(*                              if NoDuplicates_dec string_dec (map (fun x => fst (fst x)) funs) *)
+(*                              then Rval {| sev := build_rec_env funs env nsEmpty; sec := nsEmpty |} *)
+(*                              else Rerr (Rabort Rtype_error)) *)
+
+(*     | [Dtype locs tds] => if UniqueCtorsInDefs_dec tds *)
+(*                          then (state_update_next_type_stamp st (next_type_stamp st + List.length tds), *)
+(*                                Rval {| sev := nsEmpty; sec := build_tdefs (next_type_stamp st) tds |}) *)
+(*                          else (st, Rerr (Rabort Rtype_error)) *)
+    (* | [Dtabbrev locs tvs tn t] => (st, Rval {| sev := nsEmpty; sec := nsEmpty |}) *)
+    (* | [Dexn locs cn ts] => (state_update_next_exn_stamp st (next_exn_stamp st + 1), *)
+    (*                        Rval {| sev := nsEmpty; *)
+    (*                                sec := nsSing cn (List.length ts, ExnStamp (next_exn_stamp st)) |}) *)
+    (* | [Dmod mn ds] => match evaluate_decs fuel' st env ds with *)
+    (*                  | (st', r) => (st', *)
+    (*                                match r with *)
+    (*                                | Rval env' => Rval {| sev := nsLift mn (sev env'); *)
+    (*                                                      sec := nsLift mn (sec env') |} *)
+    (*                                | Rerr err => Rerr err *)
+    (*                                end) *)
+    (*                  end *)
+    (* | [Dlocal lds ds] => match evaluate_decs fuel' st env lds with *)
+    (*                     | (st1, Rval env1) => *)
+    (*                       evaluate_decs fuel' st1 (extend_dec_env env1 env) ds *)
+    (*                     | res => res *)
+    (*                     end *)
+    (* end. *)
+(* Obligation 1. *)
+
+(* unfold size_decs. simpl. *)
+
+(* assert (fold_addition_lt : forall (l : list nat) (n m : nat), n < m -> n < fold_left plus l m). *)
+(*     (induction l; intros n m H; try (specialize (IHl n (m+a))); simpl; omega). *)
+
+(* pose size_dec_min_1 as H. *)
+
+(* destruct d1; simpl; *)
+(* try (apply fold_addition_lt; *)
+(* specialize (size_dec_min_1 d2); omega). *)
+(* Qed. *)
+(* Obligation 2. *)
+(* unfold size_decs. simpl. *)
+(* assert (fold_addition_lt : forall (l : list nat) (m n : nat), m < m + n -> fold_left plus l m < fold_left plus l (m + n)). *)
+(* induction l; intros m n H. *)
+(* simpl; omega. *)
+(* simpl. rewrite <- (plus_assoc m n a). rewrite (plus_comm n a). rewrite (plus_assoc m a n). *)
+(* apply IHl. omega. *)
+
+(* rewrite plus_comm. *)
+(* apply fold_addition_lt. *)
+(* specialize (size_dec_min_1 d2). *)
+(* specialize (size_dec_min_1 d1). *)
+(* omega. *)
+(* Qed. *)
